Add correctness proof for Ford-Fulkerson algorithm

BFS/BFS.thy
@@ -1,10 +1,11 @@
 theory BFS
-imports
+  imports
+    "../Graph_Theory/Directed_Graphs/Directed_Adjacency"
     "../Map_Specs_Tbd"
     "../Misc_Tbd"
     "../Queue_Specs"
+    "../Graph_Theory/Directed_Graphs/Shortest_Dpath"
     "../Tbd"
-    "../Tbd_Graph"
 begin
 
 record ('q, 'm) state =
@@ -26,41 +27,34 @@ locale bfs =
   head = Q_head and
   tail = Q_tail and
   invar = Q_invar and
-  list = Q_list
-  for
-    Map_update :: "'a::linorder \<Rightarrow> 's \<Rightarrow> 'n \<Rightarrow> 'n" and
-    P_empty and
-    P_update :: "'a \<Rightarrow> 'a \<Rightarrow> 'm \<Rightarrow> 'm" and
-    P_delete and
-    P_lookup and
-    P_invar and
-    Q_empty and
-    Q_is_empty and
-    Q_snoc :: "'q \<Rightarrow> 'a \<Rightarrow> 'q" and
-    Q_head and
-    Q_tail and
-    Q_invar and
-    Q_list
+  list = Q_list for
+  Map_update :: "'a::linorder \<Rightarrow> 's \<Rightarrow> 'n \<Rightarrow> 'n" and
+  P_empty and
+  P_update :: "'a \<Rightarrow> 'a \<Rightarrow> 'm \<Rightarrow> 'm" and
+  P_delete and
+  P_lookup and
+  P_invar and
+  Q_empty and
+  Q_is_empty and
+  Q_snoc :: "'q \<Rightarrow> 'a \<Rightarrow> 'q" and
+  Q_head and
+  Q_tail and
+  Q_invar and
+  Q_list
 begin
 
-abbreviation dist :: "'n \<Rightarrow> 'a \<Rightarrow> 'a \<Rightarrow> enat" where
-  "dist G \<equiv> Shortest_Dpath.dist (G.E G)"
-
-abbreviation is_shortest_dpath :: "'n \<Rightarrow> 'a list \<Rightarrow> 'a \<Rightarrow> 'a \<Rightarrow> bool" where
-  "is_shortest_dpath G p u v \<equiv> dpath_bet (G.E G) p u v \<and> dpath_length p = dist G u v"
-
-section \<open>BFS algorithm\<close>
+section \<open>Algorithm\<close>
 
 definition init :: "'a \<Rightarrow> ('q, 'm) state" where
   "init src \<equiv>
    \<lparr>queue = Q_snoc Q_empty src,
     parent = P_empty\<rparr>"
 
-definition cond :: "('q, 'm) state \<Rightarrow> bool" where
-  "cond s \<longleftrightarrow> \<not> Q_is_empty (queue s)"
+definition DONE :: "('q, 'm) state \<Rightarrow> bool" where
+  "DONE s \<longleftrightarrow> Q_is_empty (queue s)"
 
-definition discovered :: "'a \<Rightarrow> ('q, 'm) state \<Rightarrow> 'a \<Rightarrow> bool" where
-  "discovered src s v \<longleftrightarrow> v = src \<or> P_lookup (parent s) v \<noteq> None"
+definition discovered :: "'a \<Rightarrow> 'm \<Rightarrow> 'a \<Rightarrow> bool" where
+  "discovered src m v \<longleftrightarrow> v = src \<or> P_lookup m v \<noteq> None"
 
 definition discover :: "'a \<Rightarrow> 'a \<Rightarrow> ('q, 'm) state \<Rightarrow> ('q, 'm) state" where
   "discover u v s \<equiv>
@@ -69,61 +63,59 @@ definition discover :: "'a \<Rightarrow> 'a \<Rightarrow> ('q, 'm) state \<Right
 
 definition traverse_edge :: "'a \<Rightarrow> 'a \<Rightarrow> 'a \<Rightarrow> ('q, 'm) state \<Rightarrow> ('q, 'm) state" where
   "traverse_edge src u v s \<equiv>
-   if \<not> discovered src s v then discover u v s
+   if \<not> discovered src (parent s) v then discover u v s
    else s"
 
 function (domintros) loop :: "'n \<Rightarrow> 'a \<Rightarrow> ('q, 'm) state \<Rightarrow> ('q, 'm) state" where
   "loop G src s =
-   (if cond s
+   (if \<not> DONE s
     then let
           u = Q_head (queue s);
           q = Q_tail (queue s)
-         in loop G src (fold (traverse_edge src u) (G.out_neighborhood G u) (s\<lparr>queue := q\<rparr>))
+         in loop G src (fold (traverse_edge src u) (G.adjacency G u) (s\<lparr>queue := q\<rparr>))
     else s)"
   by pat_completeness simp
 
-abbreviation bfs :: "'n \<Rightarrow> 'a \<Rightarrow> ('q, 'm) state" where
-  "bfs G src \<equiv> loop G src (init src)"
-
-section \<open>\<close>
+abbreviation bfs :: "'n \<Rightarrow> 'a \<Rightarrow> 'm" where
+  "bfs G src \<equiv> parent (loop G src (init src))"
 
 abbreviation fold :: "'n \<Rightarrow> 'a \<Rightarrow> ('q, 'm) state \<Rightarrow> ('q, 'm) state" where
   "fold G src s \<equiv>
    List.fold
     (traverse_edge src (Q_head (queue s)))
-    (G.out_neighborhood G (Q_head (queue s)))
+    (G.adjacency G (Q_head (queue s)))
     (s\<lparr>queue := Q_tail (queue s)\<rparr>)"
 
-abbreviation T :: "('q, 'm) state \<Rightarrow> 'a dgraph" where
-  "T s \<equiv> {(u, v) |u v. P_lookup (parent s) v = Some u}"
+abbreviation T :: "'m \<Rightarrow> 'a dgraph" where
+  "T m \<equiv> {(u, v). P_lookup m v = Some u}"
 
 section \<open>Convenience Lemmas\<close>
 
 subsection \<open>@{term "Q_invar \<circ> queue"}\<close>
 
-lemma tail_invar:
+lemma invar_tail:
   assumes "Q_invar (queue s)"
-  assumes "cond s"
+  assumes "\<not> DONE s"
   shows "Q_invar (queue (s\<lparr>queue := Q_tail (queue s)\<rparr>))"
   using assms Q.invar_tail
-  by (simp add: cond_def Q.is_empty)
+  by (simp add: DONE_def Q.is_empty)
 
 subsection \<open>@{term "Q_list \<circ> queue"}\<close>
 
 lemma list_queue_non_empty:
   assumes "Q_invar (queue s)"
-  assumes "cond s"
+  assumes "\<not> DONE s"
   shows "Q_list (queue s) \<noteq> []"
   using assms
-  by (simp add: cond_def Q.is_empty)
+  by (simp add: DONE_def Q.is_empty)
 
 subsection \<open>@{term "Q_head \<circ> queue"}\<close>
 
-lemma head_queue_mem_V:
+lemma head_queue_mem_dV:
   assumes "Q_invar (queue s)"
-  assumes "set (Q_list (queue s)) \<subseteq> G.V G"
-  assumes "cond s"
-  shows "Q_head (queue s) \<in> G.V G"
+  assumes "set (Q_list (queue s)) \<subseteq> G.dV G"
+  assumes "\<not> DONE s"
+  shows "Q_head (queue s) \<in> G.dV G"
   using assms list_queue_non_empty
   by (auto simp add: Q.list_head)
 
@@ -148,12 +140,12 @@ subsection \<open>@{term traverse_edge}\<close>
 subsubsection \<open>@{term queue}\<close>
 
 lemma queue_traverse_edge_cong:
-  shows "queue (traverse_edge src u v s) = (if \<not> discovered src s v then Q_snoc (queue s) v else queue s)"
+  shows "queue (traverse_edge src u v s) = (if \<not> discovered src (parent s) v then Q_snoc (queue s) v else queue s)"
   by (simp add: traverse_edge_def)
 
 subsubsection \<open>@{term "Q_invar \<circ> queue"}\<close>
 
-lemma queue_traverse_edge_invar:
+lemma invar_queue_traverse_edge:
   assumes "Q_invar (queue s)"
   shows "Q_invar (queue (traverse_edge src u v s))"
   using assms Q.invar_snoc
@@ -165,7 +157,7 @@ lemma list_queue_traverse_edge_cong:
   assumes "Q_invar (queue s)"
   shows
     "Q_list (queue (traverse_edge src u v s)) =
-     Q_list (queue s) @ (if \<not> discovered src s v then [v] else [])"
+     Q_list (queue s) @ (if \<not> discovered src (parent s) v then [v] else [])"
   using assms
   by (simp add: queue_traverse_edge_cong Q.list_snoc)
 
@@ -178,13 +170,13 @@ lemma lookup_parent_traverse_edge_cong:
      override_on
       (P_lookup (parent s))
       (\<lambda>_. Some u)
-      (if \<not> discovered src s v then {v} else {})"
+      (if \<not> discovered src (parent s) v then {v} else {})"
   using assms
   by (simp add: traverse_edge_def P.map_update override_on_insert')
 
 subsubsection \<open>@{term "P_invar \<circ> parent"}\<close>
 
-lemma parent_traverse_edge_invar:
+lemma invar_parent_traverse_edge:
   assumes "P_invar (parent s)"
   shows "P_invar (parent (traverse_edge src u v s))"
   using assms P.invar_update
@@ -194,7 +186,7 @@ subsubsection \<open>@{term T}\<close>
 
 lemma T_traverse_edge_cong:
   assumes "P_invar (parent s)"
-  shows "T (traverse_edge src u v s) = T s \<union> (if \<not> discovered src s v then {(u, v)} else {})"
+  shows "T (parent (traverse_edge src u v s)) = T (parent s) \<union> (if \<not> discovered src (parent s) v then {(u, v)} else {})"
   using assms
   by (auto simp add: lookup_parent_traverse_edge_cong override_on_def discovered_def)
 
@@ -202,34 +194,34 @@ subsection \<open>@{term fold}\<close>
 
 subsubsection \<open>@{term "Q_invar \<circ> queue"}\<close>
 
-lemma queue_fold_invar:
+lemma invar_queue_fold:
   assumes "Q_invar (queue s)"
   assumes "distinct l"
   shows "Q_invar (queue (List.fold (traverse_edge src u) l s))"
   using assms
-  by (induct l arbitrary: s) (simp_all add: queue_traverse_edge_invar)
+  by (induct l arbitrary: s) (simp_all add: invar_queue_traverse_edge)
 
-lemma queue_fold_invar_2:
+lemma invar_queue_fold_2:
   assumes "G.invar G"
   assumes "Q_invar (queue s)"
-  assumes "cond s"
+  assumes "\<not> DONE s"
   shows "Q_invar (queue (fold G src s))"
   using assms
-  by (auto intro: G.out_neighborhood_distinct tail_invar queue_fold_invar)
+  by (auto intro: G.distinct_adjacency invar_tail invar_queue_fold)
 
 subsubsection \<open>@{term "Q_list \<circ> queue"}\<close>
 
 lemma list_queue_fold_cong_aux:
   assumes "P_invar (parent s)"
   assumes "distinct (v # vs)"
-  shows "filter (Not \<circ> discovered src (traverse_edge src u v s)) vs = filter (Not \<circ> discovered src s) vs"
+  shows "filter (Not \<circ> discovered src (parent (traverse_edge src u v s))) vs = filter (Not \<circ> discovered src (parent s)) vs"
 proof (rule filter_cong)
   fix w
   assume "w \<in> set vs"
-  hence "discovered src (traverse_edge src u v s) w = discovered src s w"
+  hence "discovered src (parent (traverse_edge src u v s)) w = discovered src (parent s) w"
     using assms
     by (auto simp add: discovered_def lookup_parent_traverse_edge_cong override_on_insert')
-  thus "(Not \<circ> discovered src (traverse_edge src u v s)) w = (Not \<circ> discovered src s) w"
+  thus "(Not \<circ> discovered src (parent (traverse_edge src u v s))) w = (Not \<circ> discovered src (parent s)) w"
     by simp
 qed simp
 
@@ -239,7 +231,7 @@ lemma list_queue_fold_cong:
   assumes "distinct l"
   shows
     "Q_list (queue (List.fold (traverse_edge src u) l s)) =
-     Q_list (queue s) @ filter (Not \<circ> discovered src s) l"
+     Q_list (queue s) @ filter (Not \<circ> discovered src (parent s)) l"
   using assms
 proof (induct l arbitrary: s)
   case Nil
@@ -254,24 +246,24 @@ next
   also have
     "... =
      Q_list (queue (traverse_edge src u v s)) @
-     filter (Not \<circ> discovered src (traverse_edge src u v s)) vs"
+     filter (Not \<circ> discovered src (parent (traverse_edge src u v s))) vs"
     using Cons.prems
-    by (auto intro: queue_traverse_edge_invar parent_traverse_edge_invar Cons.hyps)
+    by (auto intro: invar_queue_traverse_edge invar_parent_traverse_edge Cons.hyps)
   also have
     "... =
      Q_list (queue s) @
-     (if \<not> discovered src s v then [v] else []) @
-     filter (Not \<circ> discovered src (traverse_edge src u v s)) vs"
+     (if \<not> discovered src (parent s) v then [v] else []) @
+     filter (Not \<circ> discovered src (parent (traverse_edge src u v s))) vs"
     using Cons.prems(1)
     by (simp add: list_queue_traverse_edge_cong)
   also have
     "... =
      Q_list (queue s) @
-     (if \<not> discovered src s v then [v] else []) @
-     filter (Not \<circ> discovered src s) vs"
+     (if \<not> discovered src (parent s) v then [v] else []) @
+     filter (Not \<circ> discovered src (parent s)) vs"
     using Cons.prems(2, 3)
     by (simp add: list_queue_fold_cong_aux)
-  also have "... = Q_list (queue s) @ filter (Not \<circ> discovered src s) (v # vs)"
+  also have "... = Q_list (queue s) @ filter (Not \<circ> discovered src (parent s)) (v # vs)"
     by simp
   finally show ?case
     .
@@ -281,20 +273,20 @@ lemma list_queue_fold_cong_2:
   assumes "G.invar G"
   assumes "Q_invar (queue s)"
   assumes "P_invar (parent s)"
-  assumes "cond s"
+  assumes "\<not> DONE s"
   shows
     "Q_list (queue (fold G src s)) =
      Q_list (Q_tail (queue s)) @
-     filter (Not \<circ> discovered src s) (G.out_neighborhood G (Q_head (queue s)))"
+     filter (Not \<circ> discovered src (parent s)) (G.adjacency G (Q_head (queue s)))"
 proof -
   have
     "Q_list (queue (fold G src s)) =
      Q_list (queue (s\<lparr>queue := Q_tail (queue s)\<rparr>)) @
      filter
-      (Not \<circ> discovered src (s\<lparr>queue := Q_tail (queue s)\<rparr>))
-      (G.out_neighborhood G (Q_head (queue s)))"
+      (Not \<circ> discovered src (parent (s\<lparr>queue := Q_tail (queue s)\<rparr>)))
+      (G.adjacency G (Q_head (queue s)))"
     using assms
-    by (intro tail_invar G.out_neighborhood_distinct list_queue_fold_cong) simp+
+    by (intro invar_tail G.distinct_adjacency list_queue_fold_cong) simp+
   thus ?thesis
     unfolding comp_apply
     by (simp add: discovered_def)
@@ -302,24 +294,21 @@ qed
 
 subsubsection \<open>@{term "set \<circ> Q_list \<circ> queue"}\<close>
 
-lemma queue_fold_subset_V:
+lemma queue_fold_subset_dV:
   assumes "G.invar G"
   assumes "Q_invar (queue s)"
   assumes "P_invar (parent s)"
-  assumes "set (Q_list (queue s)) \<subseteq> G.V G"
-  assumes "cond s"
-  shows "set (Q_list (queue (fold G src s))) \<subseteq> G.V G"
+  assumes "set (Q_list (queue s)) \<subseteq> G.dV G"
+  assumes "\<not> DONE s"
+  shows "set (Q_list (queue (fold G src s))) \<subseteq> G.dV G"
 proof
   fix v
   assume assm: "v \<in> set (Q_list (queue (fold G src s)))"
-  show "v \<in> G.V G"
-  proof (cases "v \<in> set (filter (Not \<circ> discovered src s) (G.out_neighborhood G (Q_head (queue s))))")
+  show "v \<in> G.dV G"
+  proof (cases "v \<in> set (filter (Not \<circ> discovered src (parent s)) (G.adjacency G (Q_head (queue s))))")
     case True
-    have "set (G.out_neighborhood G (Q_head (queue s))) \<subseteq> G.V G"
-      using assms
-      by (intro head_queue_mem_V G.out_neighborhood_subset_V)
     thus ?thesis
-      using True
+      using G.adjacency_subset_dV
       by auto
   next
     case False
@@ -345,7 +334,7 @@ lemma lookup_parent_fold_cong:
      override_on
       (P_lookup (parent s))
       (\<lambda>_. Some u)
-      (set (filter (Not \<circ> discovered src s) l))"
+      (set (filter (Not \<circ> discovered src (parent s)) l))"
   using assms
 proof (induct l arbitrary: s)
   case Nil
@@ -362,23 +351,23 @@ next
      override_on
       (P_lookup (parent (traverse_edge src u v s)))
       (\<lambda>_. Some u)
-      (set (filter (Not \<circ> discovered src (traverse_edge src u v s)) vs))"
+      (set (filter (Not \<circ> discovered src (parent (traverse_edge src u v s))) vs))"
     using Cons.prems
-    by (fastforce intro: parent_traverse_edge_invar Cons.hyps)
+    by (fastforce intro: invar_parent_traverse_edge Cons.hyps)
   also have
     "... =
      override_on
-      (override_on (P_lookup (parent s)) (\<lambda>_. Some u) (if \<not> discovered src s v then {v} else {}))
+      (override_on (P_lookup (parent s)) (\<lambda>_. Some u) (if \<not> discovered src (parent s) v then {v} else {}))
       (\<lambda>_. Some u)
-      (set (filter (Not \<circ> discovered src (traverse_edge src u v s)) vs))"
+      (set (filter (Not \<circ> discovered src (parent (traverse_edge src u v s))) vs))"
     using Cons.prems(1)
     by (simp add: lookup_parent_traverse_edge_cong)
   also have
     "... =
      override_on
-      (override_on (P_lookup (parent s)) (\<lambda>_. Some u) (if \<not> discovered src s v then {v} else {}))
+      (override_on (P_lookup (parent s)) (\<lambda>_. Some u) (if \<not> discovered src (parent s) v then {v} else {}))
       (\<lambda>_. Some u)
-      (set (filter (Not \<circ> discovered src s) vs))"
+      (set (filter (Not \<circ> discovered src (parent s)) vs))"
     using Cons.prems
     by (simp add: list_queue_fold_cong_aux)
   finally show ?case
@@ -393,49 +382,49 @@ lemma lookup_parent_fold_cong_2:
      override_on
       (P_lookup (parent s))
       (\<lambda>_. Some (Q_head (queue s)))
-      (set (filter (Not \<circ> discovered src s) (G.out_neighborhood G (Q_head (queue s)))))"
+      (set (filter (Not \<circ> discovered src (parent s)) (G.adjacency G (Q_head (queue s)))))"
 proof -
   have
     "P_lookup (parent (fold G src s)) =
      override_on
       (P_lookup (parent (s\<lparr>queue := Q_tail (queue s)\<rparr>)))
       (\<lambda>_. Some (Q_head (queue s)))
-      (set (filter (Not \<circ> discovered src (s\<lparr>queue := Q_tail (queue s)\<rparr>)) (G.out_neighborhood G (Q_head (queue s)))))"
+      (set (filter (Not \<circ> discovered src (parent (s\<lparr>queue := Q_tail (queue s)\<rparr>))) (G.adjacency G (Q_head (queue s)))))"
     using assms
-    by (intro G.out_neighborhood_distinct lookup_parent_fold_cong) simp+
+    by (intro G.distinct_adjacency lookup_parent_fold_cong) simp+
   thus ?thesis
     by (simp add: discovered_def)
 qed
 
 subsubsection \<open>@{term "P_invar \<circ> parent"}\<close>
 
-lemma parent_fold_invar:
+lemma invar_parent_fold:
   assumes "P_invar (parent s)"
   assumes "distinct l"
   shows "P_invar (parent (List.fold (traverse_edge src u) l s))"
   using assms
-  by (induct l arbitrary: s) (simp_all add: parent_traverse_edge_invar)
+  by (induct l arbitrary: s) (simp_all add: invar_parent_traverse_edge)
 
-lemma parent_fold_invar_2:
+lemma invar_parent_fold_2:
   assumes "G.invar G"
   assumes "P_invar (parent s)"
   shows "P_invar (parent (fold G src s))"
   using assms
-  by (intro G.out_neighborhood_distinct parent_fold_invar) simp+
+  by (intro G.distinct_adjacency invar_parent_fold) simp+
 
 subsubsection \<open>@{term "P.dom \<circ> parent"}\<close>
 
-lemma dom_parent_fold_subset_V:
+lemma dom_parent_fold_subset_dV:
   assumes "P_invar (parent s)"
   assumes "distinct l"
-  assumes "P.dom (parent s) \<subseteq> G.V G"
-  assumes "set l \<subseteq> G.V G"
-  shows "P.dom (parent (List.fold (traverse_edge src u) l s)) \<subseteq> G.V G"
+  assumes "P.dom (parent s) \<subseteq> G.dV G"
+  assumes "set l \<subseteq> G.dV G"
+  shows "P.dom (parent (List.fold (traverse_edge src u) l s)) \<subseteq> G.dV G"
 proof
   fix v
   assume assm: "v \<in> P.dom (parent (List.fold (traverse_edge src u) l s))"
-  show "v \<in> G.V G"
-  proof (cases "v \<in> set (filter (Not \<circ> discovered src s) l)")
+  show "v \<in> G.dV G"
+  proof (cases "v \<in> set (filter (Not \<circ> discovered src (parent s)) l)")
     case True
     thus ?thesis
       using assms(4)
@@ -454,22 +443,13 @@ proof
   qed
 qed
 
-lemma dom_parent_fold_subset_V_2:
+lemma dom_parent_fold_subset_dV_2:
   assumes "G.invar G"
-  assumes "Q_invar (queue s)"
   assumes "P_invar (parent s)"
-  assumes "set (Q_list (queue s)) \<subseteq> G.V G"
-  assumes "P.dom (parent s) \<subseteq> G.V G"
-  assumes "cond s"
-  shows "P.dom (parent (fold G src s)) \<subseteq> G.V G"
-proof -
-  have "set (G.out_neighborhood G (Q_head (queue s))) \<subseteq> G.V G"
-    using assms(2, 4, 6)
-    by (intro head_queue_mem_V G.out_neighborhood_subset_V)
-  thus ?thesis
-    using assms(1, 3, 5)
-    by (intro G.out_neighborhood_distinct dom_parent_fold_subset_V) simp+
-qed
+  assumes "P.dom (parent s) \<subseteq> G.dV G"
+  shows "P.dom (parent (fold G src s)) \<subseteq> G.dV G"
+  using assms G.adjacency_subset_dV
+  by (intro G.distinct_adjacency dom_parent_fold_subset_dV) simp+
 
 subsubsection \<open>@{term "P.ran \<circ> parent"}\<close>
 
@@ -479,11 +459,11 @@ lemma ran_parent_fold_cong:
   shows
     "P.ran (parent (fold G src s)) =
      P.ran (parent s) \<union>
-     (if set (filter (Not \<circ> discovered src s) (G.out_neighborhood G (Q_head (queue s)))) = {}
+     (if set (filter (Not \<circ> discovered src (parent s)) (G.adjacency G (Q_head (queue s)))) = {}
       then {}
       else {Q_head (queue s)})"
 proof
-  let ?S = "set (filter (Not \<circ> discovered src s) (G.out_neighborhood G (Q_head (queue s))))"
+  let ?S = "set (filter (Not \<circ> discovered src (parent s)) (G.adjacency G (Q_head (queue s))))"
   show "P.ran (parent (fold G src s)) \<subseteq> P.ran (parent s) \<union> (if ?S = {} then {} else {Q_head (queue s)})"
     using assms
     by (auto simp add: P.ran_def lookup_parent_fold_cong_2 override_on_def)
@@ -497,7 +477,7 @@ proof
       then obtain v where
         "P_lookup (parent s) v = Some u"
         by (auto simp add: P.ran_def)
-      moreover hence "discovered src s v"
+      moreover hence "discovered src (parent s) v"
         by (simp add: discovered_def)
       ultimately show ?thesis
         using assms
@@ -523,14 +503,14 @@ subsubsection \<open>@{term T}\<close>
 lemma T_fold_cong_aux:
   assumes "P_invar (parent s)"
   assumes "distinct (v # vs)"
-  shows "w \<in> set vs \<and> \<not> discovered src (traverse_edge src u v s) w \<longleftrightarrow> w \<in> set vs \<and> \<not> discovered src s w"
+  shows "w \<in> set vs \<and> \<not> discovered src (parent (traverse_edge src u v s)) w \<longleftrightarrow> w \<in> set vs \<and> \<not> discovered src (parent s) w"
   using assms
   by (auto simp add: discovered_def lookup_parent_traverse_edge_cong override_on_def)
 
 lemma T_fold_cong:
   assumes "P_invar (parent s)"
   assumes "distinct l"
-  shows "T (List.fold (traverse_edge src u) l s) = T s \<union> {(u, v) |v. v \<in> set l \<and> \<not> discovered src s v}"
+  shows "T (parent (List.fold (traverse_edge src u) l s)) = T (parent s) \<union> {(u, v) |v. v \<in> set l \<and> \<not> discovered src (parent s) v}"
   using assms
 proof (induct l arbitrary: s)
   case Nil
@@ -539,30 +519,30 @@ proof (induct l arbitrary: s)
 next
   case (Cons v vs)
   have
-    "T (List.fold (traverse_edge src u) (v # vs) s) =
-     T (List.fold (traverse_edge src u) vs (traverse_edge src u v s))"
+    "T (parent (List.fold (traverse_edge src u) (v # vs) s)) =
+     T (parent (List.fold (traverse_edge src u) vs (traverse_edge src u v s)))"
     by simp
   also have
     "... =
-     T (traverse_edge src u v s) \<union>
-     {(u, w) |w. w \<in> set vs \<and> \<not> discovered src (traverse_edge src u v s) w}"
+     T (parent (traverse_edge src u v s)) \<union>
+     {(u, w) |w. w \<in> set vs \<and> \<not> discovered src (parent (traverse_edge src u v s)) w}"
     using Cons.prems
-    by (intro parent_traverse_edge_invar Cons.hyps) simp+
+    by (intro invar_parent_traverse_edge Cons.hyps) simp+
   also have
     "... =
-     T s \<union>
-     (if \<not> discovered src s v then {(u, v)} else {}) \<union>
-     {(u, w) |w. w \<in> set vs \<and> \<not> discovered src (traverse_edge src u v s) w}"
+     T (parent s) \<union>
+     (if \<not> discovered src (parent s) v then {(u, v)} else {}) \<union>
+     {(u, w) |w. w \<in> set vs \<and> \<not> discovered src (parent (traverse_edge src u v s)) w}"
     unfolding T_traverse_edge_cong[OF Cons.prems(1)]
     by blast
   also have
     "... =
-     T s \<union>
-     (if \<not> discovered src s v then {(u, v)} else {}) \<union>
-     {(u, w) |w. w \<in> set vs \<and> \<not> discovered src s w}"
+     T (parent s) \<union>
+     (if \<not> discovered src (parent s) v then {(u, v)} else {}) \<union>
+     {(u, w) |w. w \<in> set vs \<and> \<not> discovered src (parent s) w}"
     using Cons.prems
     by (simp add: T_fold_cong_aux)
-  also have "... = T s \<union> {(u, w) |w. w \<in> set (v # vs) \<and> \<not> discovered src s w}"
+  also have "... = T (parent s) \<union> {(u, w) |w. w \<in> set (v # vs) \<and> \<not> discovered src (parent s) w}"
     by force
   finally show ?case
     .
@@ -572,19 +552,18 @@ lemma T_fold_cong_2:
   assumes "G.invar G"
   assumes "P_invar (parent s)"
   shows
-    "T (fold G src s) =
-     T s \<union>
-     {(Q_head (queue s), v) |v.
-      v \<in> set (G.out_neighborhood G (Q_head (queue s))) \<and> \<not> discovered src s v}"
+    "T (parent (fold G src s)) =
+     T (parent s) \<union>
+     {(Q_head (queue s), v) |v. v \<in> set (G.adjacency G (Q_head (queue s))) \<and> \<not> discovered src (parent s) v}"
 proof -
   have
-    "T (fold G src s) =
-     T (s\<lparr>queue := Q_tail (queue s)\<rparr>) \<union>
+    "T (parent (fold G src s)) =
+     T (parent (s\<lparr>queue := Q_tail (queue s)\<rparr>)) \<union>
      {(Q_head (queue s), v) |v.
-      v \<in> set (G.out_neighborhood G (Q_head (queue s))) \<and>
-      \<not> discovered src (s\<lparr>queue := Q_tail (queue s)\<rparr>) v}"
+      v \<in> set (G.adjacency G (Q_head (queue s))) \<and>
+      \<not> discovered src (parent (s\<lparr>queue := Q_tail (queue s)\<rparr>)) v}"
     using assms
-    by (intro G.out_neighborhood_distinct T_fold_cong) simp+
+    by (intro G.distinct_adjacency T_fold_cong) simp+
   thus ?thesis
     by (simp add: discovered_def)
 qed
@@ -594,21 +573,20 @@ section \<open>Termination\<close>
 lemma loop_dom_aux:
   assumes "G.invar G"
   assumes "P_invar (parent s)"
-  assumes "P.dom (parent s) \<subseteq> G.V G"
+  assumes "P.dom (parent s) \<subseteq> G.dV G"
   shows
     "card (P.dom (parent (fold G src s))) =
      card (P.dom (parent s)) +
-     card (set (filter (Not \<circ> discovered src s) (G.out_neighborhood G (Q_head (queue s)))))"
+     card (set (filter (Not \<circ> discovered src (parent s)) (G.adjacency G (Q_head (queue s)))))"
 proof -
-  let ?S = "set (filter (Not \<circ> discovered src s) (G.out_neighborhood G (Q_head (queue s))))"
+  let ?S = "set (filter (Not \<circ> discovered src (parent s)) (G.adjacency G (Q_head (queue s))))"
   have "P.dom (parent (fold G src s)) = P.dom (parent s) \<union> ?S"
     using assms(1, 2)
     by (auto simp add: P.dom_def lookup_parent_fold_cong_2 override_on_def)
   moreover have "finite (P.dom (parent s))"
     using assms(1, 3) finite_subset
-    by (fastforce intro: G.E_finite vertices_finite)
+    by (fastforce intro: G.finite_dV)
   moreover have "finite ?S"
-    using G.out_neighborhood_finite
     by simp
   moreover have "P.dom (parent s) \<inter> ?S = {}"
     by (auto simp add: P.dom_def discovered_def)
@@ -617,27 +595,27 @@ proof -
 qed
 
 lemma loop_dom_aux_2:
-  assumes G_invar: "G.invar G"
-  assumes queue_invar: "Q_invar (queue s)"
-  assumes cond: "cond s"
-  assumes dom_parent_subset_V: "P.dom (parent s) \<subseteq> G.V G"
+  assumes invar_G: "G.invar G"
+  assumes invar_queue: "Q_invar (queue s)"
+  assumes not_DONE: "\<not> DONE s"
+  assumes dom_parent_subset_dV: "P.dom (parent s) \<subseteq> G.dV G"
   shows
-    "card (G.V G) +
+    "card (G.dV G) +
      length (Q_list (Q_tail (queue s))) -
      card (P.dom (parent s)) <
-     card (G.V G) +
+     card (G.dV G) +
      length (Q_list (queue s)) -
      card (P.dom (parent s))"
 proof -
   have "Q_list (queue s) \<noteq> []"
-    using queue_invar cond
+    using invar_queue not_DONE
     by (intro list_queue_non_empty)
   hence "length (Q_list (Q_tail (queue s))) < length (Q_list (queue s))"
-    using queue_invar
+    using invar_queue
     by (simp add: Q.list_tail)
-  moreover have "card (P.dom (parent s)) \<le> card (G.V G)"
-    using G_invar dom_parent_subset_V
-    by (intro G.E_finite vertices_finite card_mono)
+  moreover have "card (P.dom (parent s)) \<le> card (G.dV G)"
+    using invar_G dom_parent_subset_dV
+    by (intro G.finite_dV card_mono)
   ultimately show ?thesis
     by simp
 qed
@@ -646,47 +624,47 @@ lemma loop_dom:
   assumes "G.invar G"
   assumes "Q_invar (queue s)"
   assumes "P_invar (parent s)"
-  assumes "set (Q_list (queue s)) \<subseteq> G.V G"
-  assumes "P.dom (parent s) \<subseteq> G.V G"
+  assumes "set (Q_list (queue s)) \<subseteq> G.dV G"
+  assumes "P.dom (parent s) \<subseteq> G.dV G"
   shows "loop_dom (G, src, s)"
   using assms
-proof (induct "card (G.V G) + length (Q_list (queue s)) - card (P.dom (parent s))"
+proof (induct "card (G.dV G) + length (Q_list (queue s)) - card (P.dom (parent s))"
        arbitrary: s
        rule: less_induct)
   case less
   show ?case
-  proof (cases "cond s")
+  proof (cases "DONE s")
     case True
+    thus ?thesis
+      by (blast intro: loop.domintros)
+  next
+    case False
     let ?u = "Q_head (queue s)"
     let ?q = "Q_tail (queue s)"
-    let ?S = "set (filter (Not \<circ> discovered src s) (G.out_neighborhood G (Q_head (queue s))))"
+    let ?S = "set (filter (Not \<circ> discovered src (parent s)) (G.adjacency G (Q_head (queue s))))"
 
     have "length (Q_list (queue (fold G src s))) = length (Q_list ?q) + card ?S"
-      using less.prems(1-3) True G.out_neighborhood_distinct
+      using less.prems(1-3) False G.distinct_adjacency
       by (simp add: list_queue_fold_cong_2 distinct_card[symmetric])
     moreover have "card (P.dom (parent (fold G src s))) = card (P.dom (parent s)) + card ?S"
       using less.prems(1, 3, 5)
       by (intro loop_dom_aux)
     ultimately have
-      "card (G.V G) + length (Q_list (queue (fold G src s))) - card (P.dom (parent (fold G src s))) =
-       card (G.V G) + length (Q_list ?q) + card ?S - (card (P.dom (parent s)) + card ?S)"
+      "card (G.dV G) + length (Q_list (queue (fold G src s))) - card (P.dom (parent (fold G src s))) =
+       card (G.dV G) + length (Q_list ?q) + card ?S - (card (P.dom (parent s)) + card ?S)"
       by presburger
-    also have "... = card (G.V G) + length (Q_list ?q) - card (P.dom (parent s))"
+    also have "... = card (G.dV G) + length (Q_list ?q) - card (P.dom (parent s))"
       by simp
-    also have "... < card (G.V G) + length (Q_list (queue s)) - card (P.dom (parent s))"
-      using less.prems True
+    also have "... < card (G.dV G) + length (Q_list (queue s)) - card (P.dom (parent s))"
+      using less.prems False
       by (intro loop_dom_aux_2)
     finally have
-      "card (G.V G) + length (Q_list (queue (fold G src s))) - card (P.dom (parent (fold G src s))) <
-       card (G.V G) + length (Q_list (queue s)) - card (P.dom (parent s))"
+      "card (G.dV G) + length (Q_list (queue (fold G src s))) - card (P.dom (parent (fold G src s))) <
+       card (G.dV G) + length (Q_list (queue s)) - card (P.dom (parent s))"
       .
     thus ?thesis
       using less.prems
-      by (intro queue_fold_invar_2 parent_fold_invar_2 queue_fold_subset_V dom_parent_fold_subset_V_2 less.hyps loop.domintros)
-  next
-    case False
-    thus ?thesis
-      by (blast intro: loop.domintros)
+      by (intro invar_queue_fold_2 invar_parent_fold_2 queue_fold_subset_dV dom_parent_fold_subset_dV_2 less.hyps loop.domintros)
   qed
 qed
 
@@ -694,443 +672,64 @@ end
 
 section \<open>Invariants\<close>
 
+subsection \<open>Definitions\<close>
+
+(* TODO Rename. *)
+abbreviation (in bfs) rev_follow :: "'m \<Rightarrow> 'a \<Rightarrow> 'a dpath" where
+  "rev_follow m v \<equiv> rev (parent.follow (P_lookup m) v)"
+
 locale bfs_invar_tbd = bfs where
   Map_update = Map_update and
   P_update = P_update and
-  Q_snoc = Q_snoc
-  for
-    Map_update :: "'a::linorder \<Rightarrow> 's \<Rightarrow> 'n \<Rightarrow> 'n" and
-    P_update :: "'a \<Rightarrow> 'a \<Rightarrow> 'm \<Rightarrow> 'm" and
-    Q_snoc :: "'q \<Rightarrow> 'a \<Rightarrow> 'q" +
+  Q_snoc = Q_snoc for
+  Map_update :: "'a::linorder \<Rightarrow> 's \<Rightarrow> 'n \<Rightarrow> 'n" and
+  P_update :: "'a \<Rightarrow> 'a \<Rightarrow> 'm \<Rightarrow> 'm" and
+  Q_snoc :: "'q \<Rightarrow> 'a \<Rightarrow> 'q" +
   fixes G :: 'n
   fixes src :: 'a
-  assumes G_invar: "G.invar G"
-  assumes src_mem_V: "src \<in> G.V G"
-begin
+  assumes invar_G: "G.invar G"
+  assumes src_mem_dV: "src \<in> G.dV G"
 
-subsection \<open>Convenience Lemmas\<close>
+abbreviation (in bfs_invar_tbd) d :: "'m \<Rightarrow> 'a \<Rightarrow> nat" where
+  "d m v \<equiv> dpath_length (rev_follow m v)"
 
-lemma E_finite:
-  shows "finite (G.E G)"
-  using G_invar
-  by (intro G.E_finite)
+abbreviation (in bfs_invar_tbd) white :: "('q, 'm) state \<Rightarrow> 'a \<Rightarrow> bool" where
+  "white s v \<equiv> \<not> discovered src (parent s) v"
 
-subsection \<open>\<close>
+abbreviation (in bfs_invar_tbd) gray :: "('q, 'm) state \<Rightarrow> 'a \<Rightarrow> bool" where
+  "gray s v \<equiv> discovered src (parent s) v \<and> v \<in> set (Q_list (queue s))"
 
-abbreviation white :: "('q, 'm) state \<Rightarrow> 'a \<Rightarrow> bool" where
-  "white s v \<equiv> \<not> discovered src s v"
-
-abbreviation gray :: "('q, 'm) state \<Rightarrow> 'a \<Rightarrow> bool" where
-  "gray s v \<equiv> discovered src s v \<and> v \<in> set (Q_list (queue s))"
-
-abbreviation black :: "('q, 'm) state \<Rightarrow> 'a \<Rightarrow> bool" where
-  "black s v \<equiv> discovered src s v \<and> v \<notin> set (Q_list (queue s))"
-
-lemma gray_imp_not_white:
-  assumes "gray s v"
-  shows "\<not> white s v"
-  using assms
-  by simp
-
-lemma black_imp_not_white:
-  assumes "black s v"
-  shows "\<not> white s v"
-  using assms
-  by simp
-
-lemma vertex_color_induct [case_names white gray black]:
-  assumes "white s v \<Longrightarrow> P s v"
-  assumes "gray s v \<Longrightarrow> P s v"
-  assumes "black s v \<Longrightarrow> P s v"
-  shows "P s v"
-  using assms
-  by blast
-
-end
+abbreviation (in bfs_invar_tbd) black :: "('q, 'm) state \<Rightarrow> 'a \<Rightarrow> bool" where
+  "black s v \<equiv> discovered src (parent s) v \<and> v \<notin> set (Q_list (queue s))"
 
 locale bfs_invar =
   bfs_invar_tbd where P_update = P_update and Q_snoc = Q_snoc +
-  parent "P_lookup (parent s)"
-  for
-    P_update :: "'a::linorder \<Rightarrow> 'a \<Rightarrow> 'm \<Rightarrow> 'm" and
-    Q_snoc :: "'q \<Rightarrow> 'a \<Rightarrow> 'q" and
-    s :: "('q, 'm) state" +
-  assumes queue_invar: "Q_invar (queue s)"
-  assumes queue_distinct: "distinct (Q_list (queue s))"
-  assumes parent_invar: "P_invar (parent s)"
+  parent "P_lookup (parent s)" for
+  P_update :: "'a::linorder \<Rightarrow> 'a \<Rightarrow> 'm \<Rightarrow> 'm" and
+  Q_snoc :: "'q \<Rightarrow> 'a \<Rightarrow> 'q" and
+  s :: "('q, 'm) state" +
+  assumes invar_queue: "Q_invar (queue s)"
+  assumes invar_parent: "P_invar (parent s)"
   assumes parent_src: "P_lookup (parent s) src = None"
-  assumes gray_if_mem_queue: "v \<in> set (Q_list (queue s)) \<Longrightarrow> gray s v"
-  assumes black_if_mem_ran: "v \<in> P.ran (parent s) \<Longrightarrow> black s v"
-  assumes queue_sorted_wrt_dpath_length:
-    "sorted_wrt (\<lambda>u v. dpath_length (rev (follow u)) \<le> dpath_length (rev (follow v))) (Q_list (queue s))"
-  assumes tbd_dpath_length:
-    "\<not> Q_is_empty (queue s) \<Longrightarrow>
-     dpath_length (rev (follow (last (Q_list (queue s))))) \<le> dpath_length (rev (follow (Q_head (queue s)))) + 1"
-  assumes not_white_imp_shortest_dpath:
-    "\<not> white s v \<Longrightarrow> is_shortest_dpath G (rev (follow v)) src v"
-  assumes black_imp_out_neighborhood_not_white: "black s v \<Longrightarrow> \<forall>w\<in>set (G.out_neighborhood G v). \<not> white s w"
-begin
+  assumes parent_imp_edge: "P_lookup (parent s) v = Some u \<Longrightarrow> (u, v) \<in> G.dE G"
+  assumes not_white_if_mem_queue: "v \<in> set (Q_list (queue s)) \<Longrightarrow> \<not> white s v"
+  assumes not_white_if_parent: "P_lookup (parent s) v = Some u \<Longrightarrow> \<not> white s u"
+  assumes black_imp_adjacency_not_white: "\<lbrakk> (u, v) \<in> G.dE G; black s u \<rbrakk> \<Longrightarrow> \<not> white s v"
+  assumes queue_sorted_wrt_d: "sorted_wrt (\<lambda>u v. d (parent s) u \<le> d (parent s) v) (Q_list (queue s))"
+  assumes d_last_queue_le: "\<not> Q_is_empty (queue s) \<Longrightarrow> d (parent s) (last (Q_list (queue s))) \<le> d (parent s) (Q_head (queue s)) + 1"
+  assumes d_triangle_inequality: "\<lbrakk> dpath_bet (G.dE G) p u v; \<not> white s u; \<not> white s v \<rbrakk> \<Longrightarrow> d (parent s) v \<le> d (parent s) u + dpath_length p"
 
-subsection \<open>Convenience Lemmas\<close>
+locale bfs_invar_not_DONE = bfs_invar where P_update = P_update and Q_snoc = Q_snoc for
+  P_update :: "'a::linorder \<Rightarrow> 'a \<Rightarrow> 'm \<Rightarrow> 'm" and
+  Q_snoc :: "'q \<Rightarrow> 'a \<Rightarrow> 'q" +
+  assumes not_DONE: "\<not> DONE s"
 
-lemma queue_subset_V:
-  shows "set (Q_list (queue s)) \<subseteq> G.V G"
-  using gray_if_mem_queue not_white_imp_shortest_dpath
-  by (fastforce intro: dpath_bet_endpoints(2))
+locale bfs_invar_DONE = bfs_invar where P_update = P_update and Q_snoc = Q_snoc for
+  P_update :: "'a::linorder \<Rightarrow> 'a \<Rightarrow> 'm \<Rightarrow> 'm" and
+  Q_snoc :: "'q \<Rightarrow> 'a \<Rightarrow> 'q" +
+  assumes DONE: "DONE s"
 
-lemma head_queue_mem_V:
-  assumes "cond s"
-  shows "Q_head (queue s) \<in> G.V G"
-  using queue_invar assms queue_subset_V
-  by (intro head_queue_mem_V)
-
-lemma list_queue_fold_cong:
-  assumes "cond s"
-  shows
-    "Q_list (queue (fold G src s)) =
-     Q_list (Q_tail (queue s)) @
-     filter (Not \<circ> discovered src s) (G.out_neighborhood G (Q_head (queue s)))"
-  using G_invar queue_invar parent_invar assms
-  by (intro list_queue_fold_cong_2)
-
-lemma lookup_parent_fold_cong:
-  shows
-    "P_lookup (parent (fold G src s)) =
-     override_on
-      (P_lookup (parent s))
-      (\<lambda>_. Some (Q_head (queue s)))
-      (set (filter (Not \<circ> discovered src s) (G.out_neighborhood G (Q_head (queue s)))))"
-  using G_invar parent_invar
-  by (intro lookup_parent_fold_cong_2)
-
-lemma T_fold_cong:
-  shows
-    "T (fold G src s) =
-     T s \<union>
-     {(Q_head (queue s), v) |v.
-      v \<in> set (G.out_neighborhood G (Q_head (queue s))) \<and> \<not> discovered src s v}"
-  using G_invar parent_invar
-  by (intro T_fold_cong_2)
-
-lemma src_not_white:
-  shows "\<not> white s src"
-  by (simp add: discovered_def)
-
-lemma mem_queue_imp_dpath_length_head_queue:
-  assumes "v \<in> set (Q_list (queue s))"
-  shows "dpath_length (rev (follow (Q_head (queue s)))) \<le> dpath_length (rev (follow v))"
-proof (cases "v = Q_head (queue s)")
-  case True
-  thus ?thesis
-    by simp
-next
-  case False
-  have "\<not> Q_is_empty (queue s)"
-    using queue_invar assms
-    by (auto simp add: Q.is_empty)
-  moreover hence "Q_head (queue s) = hd (Q_list (queue s))"
-    using queue_invar Q.list_head
-    by (simp add: Q.is_empty)
-  ultimately show ?thesis
-    using queue_sorted_wrt_dpath_length assms False sorted_wrt_imp_hd
-    by fastforce
-qed
-
-lemma mem_queue_imp_dist_head_queue:
-  assumes "v \<in> set (Q_list (queue s))"
-  shows "dist G src (Q_head (queue s)) \<le> dist G src v"
-proof -
-  have "Q_list (queue s) \<noteq> []"
-    using assms
-    by fastforce
-  hence "Q_head (queue s) \<in> set (Q_list (queue s))"
-    using queue_invar
-    by (simp add: Q.list_head)
-  hence "dist G src (Q_head (queue s)) = dpath_length (rev (follow (Q_head (queue s))))"
-    using gray_if_mem_queue not_white_imp_shortest_dpath
-    by force
-  also have "... \<le> dpath_length (rev (follow v))"
-    using assms
-    by (auto intro: mem_queue_imp_dpath_length_head_queue)
-  also have "... = dist G src v"
-    using assms gray_if_mem_queue
-    by (simp add: not_white_imp_shortest_dpath)
-  finally show ?thesis
-    .
-qed
-
-lemma mem_queue_imp_dpath_length_last_queue:
-  assumes "v \<in> set (Q_list (queue s))"
-  shows "dpath_length (rev (follow v)) \<le> dpath_length (rev (follow (last (Q_list (queue s)))))"
-proof (cases "v = last (Q_list (queue s))")
-  case True
-  thus ?thesis
-    by simp
-next
-  case False
-  have "\<not> Q_is_empty (queue s)"
-    using queue_invar assms
-    by (auto simp add: Q.is_empty)
-  thus ?thesis
-    using queue_sorted_wrt_dpath_length assms False sorted_wrt_imp_last
-    by fastforce
-qed
-
-lemma mem_queue_imp_dist_last_queue:
-  assumes "v \<in> set (Q_list (queue s))"
-  shows "dist G src v \<le> dist G src (last (Q_list (queue s)))"
-proof -
-  have list_queue_non_empty: "Q_list (queue s) \<noteq> []"
-    using assms
-    by fastforce
-  have "dist G src v = dpath_length (rev (follow v))"
-    using assms gray_if_mem_queue not_white_imp_shortest_dpath
-    by force
-  also have "... \<le> dpath_length (rev (follow (last (Q_list (queue s)))))"
-    using assms
-    by (auto intro: mem_queue_imp_dpath_length_last_queue)
-  also have "... = dist G src (last (Q_list (queue s)))"
-    using list_queue_non_empty gray_if_mem_queue
-    by (simp add: not_white_imp_shortest_dpath)
-  finally show ?thesis
-    .
-qed
-
-lemma mem_queue_dpath_lengthI:
-  assumes "v \<in> set (Q_list (queue s))"
-  shows
-    "dpath_length (rev (follow (Q_head (queue s)))) \<le> dpath_length (rev (follow v))"
-    "dpath_length (rev (follow v)) \<le> dpath_length (rev (follow (last (Q_list (queue s)))))"
-  using assms
-  by (auto intro: mem_queue_imp_dpath_length_head_queue mem_queue_imp_dpath_length_last_queue)
-
-lemma mem_queue_distI:
-  assumes "v \<in> set (Q_list (queue s))"
-  shows
-    "dist G src (Q_head (queue s)) \<le> dist G src v"
-    "dist G src v \<le> dist G src (last (Q_list (queue s)))"
-  using assms
-  by (auto intro: mem_queue_imp_dist_head_queue mem_queue_imp_dist_last_queue)
-
-subsection \<open>Basic Lemmas\<close>
-
-lemma parent_imp_edge:
-  assumes "P_lookup (parent s) v = Some u"
-  shows "(u, v) \<in> (G.E G)"
-proof -
-  have "rev (follow v) = rev (follow u) @ [v]"
-    using assms
-    by (simp add: follow_psimps)
-  moreover have "rev (follow u) = (rev (tl (follow u))) @ [u]"
-    using follow_non_empty hd_Cons_tl follow_ConsD rev.simps(2)
-    by metis
-  ultimately have "rev (follow v) = rev (tl (follow u)) @ [u, v]"
-    by simp
-  moreover have "dpath_bet (G.E G) (rev (follow v)) src v"
-    using assms not_white_imp_shortest_dpath
-    thm discovered_def
-    by (simp add: discovered_def)
-  ultimately have "dpath_bet (G.E G) (rev (tl (follow u)) @ [u, v]) src v"
-    by simp
-  thus ?thesis
-    by (auto simp add: edge_iff_dpath_bet intro: split_dpath)
-qed
-
-lemma dom_parent_subset_V:
-  shows "P.dom (parent s) \<subseteq> G.V G"
-proof
-  fix v
-  assume "v \<in> P.dom (parent s)"
-  then obtain u where
-    "P_lookup (parent s) v = Some u"
-    by (auto simp add: P.dom_def)
-  hence "(u, v) \<in> (G.E G)"
-    by (intro parent_imp_edge)
-  thus "v \<in> G.V G"
-    by (intro G.edgeI(2))
-qed
-
-lemma queue_sorted_wrt_dist:
-  shows "sorted_wrt (\<lambda>u v. dist G src u \<le> dist G src v) (Q_list (queue s))"
-proof -
-  have "\<forall>v\<in>set (Q_list (queue s)). dpath_length (rev (follow v)) = dist G src v"
-    using gray_if_mem_queue not_white_imp_shortest_dpath
-    by blast
-  hence
-    "\<And>u v. u \<in> set (Q_list (queue s)) \<Longrightarrow>
-            v \<in> set (Q_list (queue s)) \<Longrightarrow>
-            dpath_length (rev (follow u)) \<le> dpath_length (rev (follow v)) \<Longrightarrow>
-            (\<lambda>u v. dist G src u \<le> dist G src v) u v"
-    by (simp add: enat_ord_simps(1)[symmetric])
-  thus ?thesis
-    using queue_sorted_wrt_dpath_length sorted_wrt_mono_rel[of "(Q_list (queue s))"]
-    by presburger
-qed
-
-lemma tbd_dist:
-  assumes "\<not> Q_is_empty (queue s)"
-  shows "dist G src (last (Q_list (queue s))) \<le> dist G src (Q_head (queue s)) + 1"
-proof -
-  have "\<forall>v\<in>set (Q_list (queue s)). dpath_length (rev (follow v)) = dist G src v"
-    using gray_if_mem_queue not_white_imp_shortest_dpath
-    by blast
-  moreover have
-    "last (Q_list (queue s)) \<in> set (Q_list (queue s))"
-    "Q_head (queue s) \<in> set (Q_list (queue s))"
-    using queue_invar assms
-    by (simp_all add: Q.is_empty Q.list_head)
-  ultimately show ?thesis
-    using assms tbd_dpath_length
-    unfolding enat_ord_simps(1)[symmetric] plus_enat_simps(1)[symmetric] one_enat_def[symmetric]
-    by simp
-qed
-
-lemma white_imp_gray_ancestor:
-  assumes "dpath_bet (G.E G) p u v"
-  assumes "\<not> white s u"
-  assumes "white s v"
-  shows "\<exists>v\<in>set p. gray s v"
-  using assms
-proof (induct p arbitrary: v rule: dpath_rev_induct)
-  case 1
-  thus ?case
-    by simp
-next
-  case (2 w)
-  hence "[w] = [u] \<and> u = v"
-    by (intro hd_of_dpath_bet' last_of_dpath_bet list_length_1) simp
-  thus ?case
-    using "2.prems"(2, 3)
-    by simp
-next
-  case (3 w w' l)
-  show ?case
-  proof (induct s w rule: vertex_color_induct)
-    case white
-    have "dpath_bet (G.E G) (l @ [w]) u w"
-      using "3.prems"(1)
-      by (intro dpath_bet_pref) simp
-    hence "\<exists>v\<in>set (l @ [w]). gray s v"
-      using "3.prems"(2) white
-      by (intro "3.hyps")
-    thus ?thesis
-      by auto
-  next
-    case gray
-    thus ?thesis
-      by simp
-  next
-    case black
-    have "v \<in> set (G.out_neighborhood G w)"
-      using "3.prems"(1)
-      by (auto simp add: dpath_bet_def G.mem_out_neighborhood_iff_edge intro: dpath_snoc_edge_2)
-    hence "\<not> white s v"
-      using black black_imp_out_neighborhood_not_white
-      by blast
-    thus ?thesis
-      using "3.prems"(3)
-      by simp
-  qed
-qed
-
-lemma white_imp_dist_ge_case_1_subcase_3:
-  assumes IH:
-    "\<And>v. \<lbrakk> dpath_bet (G.E G) (l @ [u]) src v \<and> dpath_length (l @ [u]) = dist G src v; white s v \<rbrakk> \<Longrightarrow>
-          (if Q_is_empty (queue s) then \<infinity> else dist G src (last (Q_list (queue s)))) \<le> dist G src v"
-  assumes shortest_dpath: "is_shortest_dpath G (l @ [u, u']) src v"
-  assumes white: "white s v"
-  shows "(if Q_is_empty (queue s) then \<infinity> else dist G src (last (Q_list (queue s)))) \<le> dist G src v"
-proof (induct s u rule: vertex_color_induct)
-  case white
-  have l_Q_snoc_u_shortest_dpath: "is_shortest_dpath G (l @ [u]) src u"
-    using G_invar shortest_dpath
-    by
-      (auto
-        simp add: dpath_length_eq_dpath_weight dist_eq_\<delta> is_shortest_dpath_def[symmetric]
-        intro: G.E_finite shortest_dpath_prefix_is_shortest_dpath)
-  hence "(if Q_is_empty (queue s) then \<infinity> else dist G src (last (Q_list (queue s)))) \<le> dist G src u"
-    using white
-    by (intro IH)
-  also have "... = dpath_length (l @ [u])"
-    by (simp add: l_Q_snoc_u_shortest_dpath)
-  also have "... \<le> dpath_length (l @ [u, u'])"
-    using dpath_length_append[where ?p = "l @ [u]" and ?q = "[u']"]
-    by simp
-  also have "... = dist G src v"
-    by (simp add: shortest_dpath)
-  finally show ?case
-    .
-next
-  case gray
-  hence "\<exists>v\<in>set (l @ [u, u']). gray s v"
-    using src_not_white shortest_dpath white
-    by (blast intro: white_imp_gray_ancestor)
-  hence queue_non_empty: "\<not> Q_is_empty (queue s)"
-    using queue_invar
-    by (auto simp add: Q.is_empty)
-  hence "dist G src (last (Q_list (queue s))) \<le> dist G src (Q_head (queue s)) + 1"
-    by (intro tbd_dist)
-  also have "... \<le> dist G src u + 1"
-    using gray
-    by (blast intro: mem_queue_imp_dist_head_queue add_right_mono)
-  also have "... = dist G src v"
-    using G_invar shortest_dpath
-    by (auto intro: G.E_finite shortest_dpathE_2)
-  finally show ?case
-    using queue_non_empty
-    by simp
-next
-  case black
-  have "v \<in> set (G.out_neighborhood G u)"
-    using shortest_dpath
-    by (auto simp add: dpath_bet_def G.mem_out_neighborhood_iff_edge intro: dpath_snoc_edge_2)
-  hence "\<not> white s v"
-    using black black_imp_out_neighborhood_not_white
-    by blast
-  thus ?case
-    using white
-    by simp
-qed
-
-lemma white_imp_dist_ge:
-  assumes "white s v"
-  shows "(if Q_is_empty (queue s) then \<infinity> else dist G src (last (Q_list (queue s)))) \<le> dist G src v"
-proof (cases "reachable (G.E G) src v")
-  case True
-  then obtain p where
-    "dpath_bet (G.E G) p src v \<and> dpath_length p = dist G src v"
-    using E_finite
-    by (elim dist_dpath_betE) simp+
-  thus ?thesis
-    using assms
-  proof (induct p arbitrary: v rule: dpath_rev_induct)
-    case 1
-    thus ?case
-      by simp
-  next
-    case (2 u)
-    hence "[u] = [src] \<and> src = v"
-      by (intro hd_of_dpath_bet' last_of_dpath_bet list_length_1) auto
-    thus ?case
-      using src_not_white "2.prems"(2)
-      by simp
-  next
-    case (3 u u' l)
-    thus ?case
-      by (rule white_imp_dist_ge_case_1_subcase_3)
-  qed
-next
-  case False
-  hence "dist G src v = \<infinity>"
-    unfolding dist_eq_\<delta>
-    by (meson \<delta>_reachable_conv)
-  thus ?thesis
-    by simp
-qed
-
-end
-
-abbreviation (in bfs) bfs_invar_tbd' :: "'n \<Rightarrow> 'a \<Rightarrow> bool"  where
+abbreviation (in bfs) bfs_invar_tbd' :: "'n \<Rightarrow> 'a \<Rightarrow> bool" where
   "bfs_invar_tbd' G src \<equiv>
    bfs_invar_tbd
     Map_empty Map_delete Map_lookup Map_inorder Map_inv
@@ -1139,7 +738,7 @@ abbreviation (in bfs) bfs_invar_tbd' :: "'n \<Rightarrow> 'a \<Rightarrow> bool"
     Q_empty Q_is_empty Q_head Q_tail Q_invar Q_list
     Map_update P_update Q_snoc G src"
 
-abbreviation (in bfs) bfs_invar' :: "'n \<Rightarrow> 'a \<Rightarrow> ('q, 'm) state \<Rightarrow> bool"  where
+abbreviation (in bfs) bfs_invar' :: "'n \<Rightarrow> 'a \<Rightarrow> ('q, 'm) state \<Rightarrow> bool" where
   "bfs_invar' G src s \<equiv>
    bfs_invar
     Map_empty Map_delete Map_lookup Map_inorder Map_inv
@@ -1148,8 +747,220 @@ abbreviation (in bfs) bfs_invar' :: "'n \<Rightarrow> 'a \<Rightarrow> ('q, 'm) 
     Q_empty Q_is_empty Q_head Q_tail Q_invar Q_list
     Map_update G src P_update Q_snoc s"
 
-abbreviation (in bfs_invar_tbd) bfs_invar'' :: "('q, 'm) state \<Rightarrow> bool"  where
+abbreviation (in bfs_invar_tbd) bfs_invar'' :: "('q, 'm) state \<Rightarrow> bool" where
   "bfs_invar'' \<equiv> bfs_invar' G src"
+
+abbreviation (in bfs) bfs_invar_not_DONE' :: "'n \<Rightarrow> 'a \<Rightarrow> ('q, 'm) state \<Rightarrow> bool" where
+  "bfs_invar_not_DONE' G src s \<equiv>
+   bfs_invar_not_DONE
+    Map_empty Map_delete Map_lookup Map_inorder Map_inv
+    Set_empty Set_insert Set_delete Set_isin Set_inorder Set_inv
+    P_empty P_delete P_lookup P_invar
+    Q_empty Q_is_empty Q_head Q_tail Q_invar Q_list
+    Map_update G src s P_update Q_snoc"
+
+abbreviation (in bfs_invar_tbd) bfs_invar_not_DONE'' :: "('q, 'm) state \<Rightarrow> bool" where
+  "bfs_invar_not_DONE'' \<equiv> bfs_invar_not_DONE' G src"
+
+abbreviation (in bfs) bfs_invar_DONE' :: "'n \<Rightarrow> 'a \<Rightarrow> ('q, 'm) state \<Rightarrow> bool" where
+  "bfs_invar_DONE' G src s \<equiv>
+   bfs_invar_DONE
+    Map_empty Map_delete Map_lookup Map_inorder Map_inv
+    Set_empty Set_insert Set_delete Set_isin Set_inorder Set_inv
+    P_empty P_delete P_lookup P_invar
+    Q_empty Q_is_empty Q_head Q_tail Q_invar Q_list
+    Map_update G src s P_update Q_snoc"
+
+abbreviation (in bfs_invar_tbd) bfs_invar_DONE'' :: "('q, 'm) state \<Rightarrow> bool" where
+  "bfs_invar_DONE'' \<equiv> bfs_invar_DONE' G src"
+
+subsection \<open>Convenience Lemmas\<close>
+
+subsubsection \<open>@{term bfs}\<close>
+
+lemma (in bfs) bfs_invar_not_DONE'I:
+  assumes "bfs_invar' G src s"
+  assumes "\<not> DONE s"
+  shows "bfs_invar_not_DONE' G src s"
+  using assms
+  by (simp add: bfs_invar_not_DONE_def bfs_invar_not_DONE_axioms_def)
+
+lemma (in bfs) bfs_invar_DONE'I:
+  assumes "bfs_invar' G src s"
+  assumes "DONE s"
+  shows "bfs_invar_DONE' G src s"
+  using assms
+  by (simp add: bfs_invar_DONE_def bfs_invar_DONE_axioms_def)
+
+lemma (in bfs) rev_follow_non_empty:
+  assumes "Tbd.parent (P_lookup m)"
+  shows "rev_follow m v \<noteq> []"
+  using assms
+  by (auto dest: parent.follow_non_empty)
+
+lemma (in bfs) distinct_rev_follow:
+  assumes "Tbd.parent (P_lookup m)"
+  shows "distinct (rev_follow m v)"
+  unfolding distinct_rev
+  using assms
+  by (intro parent.distinct_follow)
+
+lemma (in bfs) last_rev_follow:
+  assumes "Tbd.parent (P_lookup m)"
+  shows "last (rev_follow m v) = v"
+proof -
+  let ?l = "parent.follow (P_lookup m) v"
+  have "?l = hd ?l # tl ?l"
+    using assms
+    by (intro parent.follow_non_empty hd_Cons_tl[symmetric])
+  hence "hd ?l = v"
+    using assms
+    by (auto dest: parent.follow_ConsD)
+  thus ?thesis
+    using assms parent.follow_non_empty
+    by (fastforce simp add: last_rev)
+qed
+
+subsubsection \<open>@{term bfs_invar_tbd}\<close>
+
+context bfs_invar_tbd
+begin
+sublocale finite_dgraph "G.dE G"
+proof (standard, goal_cases)
+  case 1
+  show ?case
+    using invar_G
+    by (intro G.finite_dE)
+qed
+end
+
+lemma (in bfs_invar_tbd) vertex_color_induct [case_names white gray black]:
+  assumes "white s v \<Longrightarrow> P s v"
+  assumes "gray s v \<Longrightarrow> P s v"
+  assumes "black s v \<Longrightarrow> P s v"
+  shows "P s v"
+  using assms
+  by blast
+
+lemma (in bfs_invar_tbd) src_not_white:
+  shows "\<not> white s src"
+  by (simp add: discovered_def)
+
+subsubsection \<open>@{term bfs_invar}\<close>
+
+lemma (in bfs_invar) distinct_rev_follow:
+  shows "distinct (rev_follow (parent s) v)"
+  using distinct_follow
+  by simp
+
+subsection \<open>Basic Lemmas\<close>
+
+subsubsection \<open>@{term bfs_invar_tbd}\<close>
+
+lemma (in bfs_invar_tbd) parent_imp_d:
+  assumes "Tbd.parent (P_lookup (parent s))"
+  assumes "P_lookup (parent s) v = Some u"
+  shows "d (parent s) v = d (parent s) u + 1"
+proof -
+  have "rev_follow (parent s) v = rev_follow (parent s) u @ [v]"
+    using assms
+    by (simp add: parent.follow_psimps)
+  thus ?thesis
+    using parent.follow_non_empty[OF assms(1)]
+    by (simp add: dpath_length_snoc)
+qed
+
+subsubsection \<open>@{term bfs_invar}\<close>
+
+lemma (in bfs_invar) not_white_imp_dpath_rev_follow:
+  assumes "\<not> white s v"
+  shows "dpath_bet (G.dE G) (rev_follow (parent s) v) src v"
+  using assms
+proof (induct v rule: follow_pinduct)
+  case (1 v)
+  show ?case
+  proof (cases "v = src")
+    case True
+    thus ?thesis
+      using parent_src src_mem_dV
+      by (auto simp add: follow_psimps intro: dpath_bet_reflexive)
+  next
+    case False
+    then obtain u where
+      u: "P_lookup (parent s) v = Some u"
+      using "1.prems"
+      by (auto simp add: discovered_def)
+    hence
+      "follow v = v # follow u"
+      "(u, v) \<in> G.dE G"
+      "\<not> white s u"
+      using not_white_if_parent
+      by (auto simp add: follow_psimps intro: parent_imp_edge)
+    moreover hence "dpath_bet (G.dE G) (rev_follow (parent s) u) src u"
+      using u
+      by (intro "1.hyps")
+    ultimately show ?thesis
+      by (auto intro: dpath_bet_snoc_edge)
+  qed
+qed
+
+lemma (in bfs_invar) hd_rev_follow_eq_src:
+  assumes "\<not> white s v"
+  shows "hd (rev_follow (parent s) v) = src"
+  using assms
+  by (intro hd_of_dpath_bet'[symmetric]) (rule not_white_imp_dpath_rev_follow)
+
+lemma (in bfs_invar) mem_queue_imp_d_ge:
+  assumes "v \<in> set (Q_list (queue s))"
+  shows "d (parent s) (Q_head (queue s)) \<le> d (parent s) v"
+proof (cases "v = Q_head (queue s)")
+  case True
+  thus ?thesis
+    by simp
+next
+  case False
+  have "\<not> Q_is_empty (queue s)"
+    using invar_queue assms
+    by (auto simp add: Q.is_empty)
+  moreover hence "Q_head (queue s) = hd (Q_list (queue s))"
+    using invar_queue Q.list_head
+    by (simp add: Q.is_empty)
+  ultimately show ?thesis
+    using queue_sorted_wrt_d assms False sorted_wrt_imp_hd
+    by fastforce
+qed
+
+lemma (in bfs_invar) mem_queue_imp_d_le:
+  assumes "v \<in> set (Q_list (queue s))"
+  shows "d (parent s) v \<le> d (parent s) (last (Q_list (queue s)))"
+proof (cases "v = last (Q_list (queue s))")
+  case True
+  thus ?thesis
+    by simp
+next
+  case False
+  have "\<not> Q_is_empty (queue s)"
+    using invar_queue assms
+    by (auto simp add: Q.is_empty)
+  thus ?thesis
+    using queue_sorted_wrt_d assms False sorted_wrt_imp_last
+    by fastforce
+qed
+
+lemma (in bfs_invar) d_triangle_inequality_edge:
+  assumes "(u, v) \<in> G.dE G"
+  assumes "\<not> white s u"
+  assumes "\<not> white s v"
+  shows "d (parent s) v \<le> d (parent s) u + 1"
+proof -
+  have "dpath_bet (G.dE G) [u, v] u v"
+    using assms(1)
+    by (intro edges_are_dpath_bet)
+  thus ?thesis
+    using assms(2, 3)
+    using d_triangle_inequality
+    by fastforce
+qed
 
 subsection \<open>@{term bfs.init}\<close>
 
@@ -1160,30 +971,18 @@ lemma (in bfs_invar_tbd) follow_invar'_parent_init:
   using wf_empty
   by (simp add: init_def P.map_empty follow_invar'_def)
 
-lemma (in bfs_invar_tbd) parent_init:
-  shows "Tbd.parent (P_lookup (parent (init src)))"
-  using follow_invar'_parent_init
-  by unfold_locales
+subsubsection \<open>@{thm bfs_invar.invar_queue}\<close>
 
-subsubsection \<open>@{thm bfs_invar.queue_invar}\<close>
-
-lemma (in bfs_invar_tbd) queue_invar_init:
+lemma (in bfs_invar_tbd) invar_queue_init:
   shows "Q_invar (queue (init src))"
   using Q.invar_empty
   by (auto simp add: init_def intro: Q.invar_snoc)
 
-subsubsection \<open>@{thm bfs_invar.queue_distinct}\<close>
+subsubsection \<open>@{thm bfs_invar.invar_parent}\<close>
 
-lemma (in bfs_invar_tbd) queue_distinct_init:
-  shows "distinct (Q_list (queue (init src)))"
-  using Q.invar_empty
-  by (simp add: init_def Q.list_snoc Q.list_empty)
-
-subsubsection \<open>@{thm bfs_invar.parent_invar}\<close>
-
-lemma (in bfs_invar_tbd) parent_invar_init:
+lemma (in bfs_invar_tbd) invar_parent_init:
   shows "P_invar (parent (init src))"
-  using P.map_specs(4)
+  using P.invar_empty
   by (simp add: init_def)
 
 subsubsection \<open>@{thm bfs_invar.parent_src}\<close>
@@ -1192,161 +991,232 @@ lemma (in bfs_invar_tbd) parent_src_init:
   shows "P_lookup (parent (init src)) src = None"
   by (simp add: init_def P.map_empty)
 
-subsubsection \<open>@{thm bfs_invar.gray_if_mem_queue}\<close>
+subsubsection \<open>@{thm bfs_invar.parent_imp_edge}\<close>
 
-lemma (in bfs_invar_tbd) gray_if_mem_queue_init:
+lemma (in bfs_invar_tbd) parent_imp_edge_init:
+  assumes "P_lookup (parent (init src)) v = Some u"
+  shows "(u, v) \<in> G.dE G"
+  using assms
+  by (simp add: init_def P.map_empty)
+
+subsubsection \<open>@{thm bfs_invar.not_white_if_mem_queue}\<close>
+
+lemma (in bfs_invar_tbd) not_white_if_mem_queue_init:
   assumes "v \<in> set (Q_list (queue (init src)))"
-  shows "gray (init src) v"
+  shows "\<not> white (init src) v"
   using assms Q.invar_empty
   by (simp add: init_def Q.list_snoc Q.list_empty discovered_def)
 
-subsubsection \<open>@{thm bfs_invar.black_if_mem_ran}\<close>
+subsubsection \<open>@{thm bfs_invar.not_white_if_parent}\<close>
 
-lemma (in bfs_invar_tbd) black_if_mem_ran_init:
-  assumes "v \<in> P.ran (parent (init src))"
-  shows "black (init src) v"
+lemma (in bfs_invar_tbd) not_white_if_parent_init:
+  assumes "P_lookup (parent (init src)) v = Some u"
+  shows "\<not> white (init src) u"
   using assms
-  by (simp add: init_def P.ran_def P.map_empty)
+  by (simp add: init_def P.map_empty)
 
-subsubsection \<open>@{thm bfs_invar.queue_sorted_wrt_dpath_length}\<close>
+subsubsection \<open>@{thm bfs_invar.black_imp_adjacency_not_white}\<close>
 
-lemma (in bfs_invar_tbd) queue_sorted_wrt_dpath_length_init:
-  shows
-    "sorted_wrt
-      (\<lambda>u v. dpath_length (rev (parent.follow (P_lookup (parent (init src))) u)) \<le>
-             dpath_length (rev (parent.follow (P_lookup (parent (init src))) v)))
-      (Q_list (queue (init src)))"
+lemma (in bfs_invar_tbd) black_imp_adjacency_not_white_init:
+  assumes "black (init src) u"
+  assumes "(u, v) \<in> G.dE G"
+  shows "\<not> white s v"
+proof -
+  have "u = src"
+    using assms(1)
+    by (simp add: discovered_def init_def P.map_empty)
+  thus ?thesis
+    using assms(1) Q.invar_empty
+    by (simp add: init_def Q.list_snoc)
+qed
+
+subsubsection \<open>@{thm bfs_invar.queue_sorted_wrt_d}\<close>
+
+lemma (in bfs_invar_tbd) queue_sorted_wrt_d_init:
+  shows "sorted_wrt (\<lambda>u v. d (parent (init src)) u \<le> d (parent (init src)) v) (Q_list (queue (init src)))"
   using Q.invar_empty
   by (simp add: init_def Q.list_snoc Q.list_empty)
 
-subsubsection \<open>@{thm bfs_invar.tbd_dpath_length}\<close>
+subsubsection \<open>@{thm bfs_invar.d_last_queue_le}\<close>
 
-lemma (in bfs_invar_tbd) tbd_dpath_length_init:
+lemma (in bfs_invar_tbd) d_last_queue_le_init:
   assumes "\<not> Q_is_empty (queue (init src))"
-  shows
-    "dpath_length (rev (parent.follow (P_lookup (parent (init src))) (last (Q_list (queue (init src)))))) \<le>
-     dpath_length (rev (parent.follow (P_lookup (parent (init src))) (Q_head (queue (init src))))) + 1"
-  using Q.invar_empty queue_invar_init
+  shows "d (parent (init src)) (last (Q_list (queue (init src)))) \<le> d (parent (init src)) (Q_head (queue (init src))) + 1"
+  using Q.invar_empty invar_queue_init
   by (simp add: init_def Q.list_snoc Q.list_empty Q.list_head)
 
-subsubsection \<open>@{thm bfs_invar.not_white_imp_shortest_dpath}\<close>
+subsubsection \<open>@{thm bfs_invar.d_triangle_inequality}\<close>
 
-lemma (in bfs_invar_tbd) not_white_imp_shortest_dpath_init:
+lemma (in bfs_invar_tbd) d_triangle_inequality_init:
+  assumes "dpath_bet (G.dE G) p u v"
+  assumes "\<not> white (init src) u"
   assumes "\<not> white (init src) v"
-  shows "is_shortest_dpath G (rev (parent.follow (P_lookup (parent (init src))) v)) src v"
-proof -
-  have dpath_bet: "dpath_bet (G.E G) [src] src src"
-    using src_mem_V
-    by (auto intro: dpath_bet_reflexive)
-  have "dpath_length [src] = 0"
-    by simp
-  also have "... \<le> dist G src src"
-    using zero_le
-    by (subst zero_enat_def[symmetric])
-  finally have "dpath_length [src] \<le> dist G src src"
-    .
-  hence "dpath_length [src] = dist G src src"
-    using E_finite dpath_bet
-    by (intro dist_le_dpath_length antisym)
-  moreover have "v = src"
-    using assms
-    by (simp add: discovered_def init_def P.map_empty)
-  moreover have "rev (parent.follow (P_lookup (parent (init src))) src) = [src]"
-    using parent_init
-    by (simp add: parent_src_init parent.follow_psimps)
-  ultimately show ?thesis
-    using dpath_bet
-    by simp
-qed
-
-subsubsection \<open>@{thm bfs_invar.black_imp_out_neighborhood_not_white}\<close>
-
-lemma (in bfs_invar_tbd) black_imp_out_neighborhood_not_white_init:
-  assumes "black (init src) v"
-  shows "\<forall>w\<in>set (G.out_neighborhood G v). \<not> white (init src) w"
-proof -
-  have "v = src"
-    using assms
-    by (simp add: discovered_def init_def P.map_empty)
-  moreover have "src \<in> set (Q_list (queue (init src)))"
-    using Q.invar_empty
-    by (simp add: init_def Q.list_snoc)
-  ultimately show ?thesis
-    using assms
-    by blast
-qed
+  shows "d (parent (init src)) v \<le> d (parent (init src)) u + dpath_length p"
+  using assms
+  by (simp add: discovered_def init_def P.map_empty)
 
 subsubsection \<open>\<close>
 
 lemma (in bfs_invar_tbd) bfs_invar_init:
   shows "bfs_invar'' (init src)"
-  using bfs_axioms
-  using follow_invar'_parent_init
-  using queue_invar_init queue_distinct_init parent_invar_init parent_src_init
-  using gray_if_mem_queue_init black_if_mem_ran_init queue_sorted_wrt_dpath_length_init tbd_dpath_length_init
-  using not_white_imp_shortest_dpath_init black_imp_out_neighborhood_not_white_init
-  by unfold_locales
+proof (standard, goal_cases)
+  case 1
+  show ?case using follow_invar'_parent_init .
+next
+  case 2
+  show ?case using invar_queue_init .
+next
+  case 3
+  show ?case using invar_parent_init .
+next
+  case 4
+  show ?case using parent_src_init .
+next
+  case (5 v u)
+  thus ?case by (intro parent_imp_edge_init)
+next
+  case (6 v)
+  thus ?case by (intro not_white_if_mem_queue_init)
+next
+  case (7 v u)
+  thus ?case by (intro not_white_if_parent_init)
+next
+  case (8 u v)
+  thus ?case by (intro black_imp_adjacency_not_white_init)
+next
+  case 9
+  show ?case using queue_sorted_wrt_d_init .
+next
+  case 10
+  thus ?case by (intro d_last_queue_le_init)
+next
+  case (11 p u v)
+  thus ?case by (intro d_triangle_inequality_init)
+qed
 
 subsection \<open>@{term bfs.fold}\<close>
 
 subsubsection \<open>Convenience Lemmas\<close>
 
-lemma (in bfs_invar) list_queue_non_empty:
-  assumes "cond s"
+lemma (in bfs_invar_not_DONE) list_queue_fold_cong:
+  shows
+    "Q_list (queue (fold G src s)) =
+     Q_list (Q_tail (queue s)) @
+     filter (Not \<circ> discovered src (parent s)) (G.adjacency G (Q_head (queue s)))"
+  using invar_G invar_queue invar_parent not_DONE
+  by (intro list_queue_fold_cong_2)
+
+lemma (in bfs_invar) lookup_parent_fold_cong:
+  shows
+    "P_lookup (parent (fold G src s)) =
+     override_on
+      (P_lookup (parent s))
+      (\<lambda>_. Some (Q_head (queue s)))
+      (set (filter (Not \<circ> discovered src (parent s)) (G.adjacency G (Q_head (queue s)))))"
+  using invar_G invar_parent
+  by (intro lookup_parent_fold_cong_2)
+
+lemma (in bfs_invar) T_fold_cong:
+  shows
+    "T (parent (fold G src s)) =
+     T (parent s) \<union>
+     {(Q_head (queue s), v) |v. v \<in> set (G.adjacency G (Q_head (queue s))) \<and> \<not> discovered src (parent s) v}"
+  using invar_G invar_parent
+  by (intro T_fold_cong_2)
+
+lemma (in bfs_invar_not_DONE) list_queue_non_empty:
   shows "Q_list (queue s) \<noteq> []"
-  using queue_invar assms
+  using invar_queue not_DONE
   by (intro list_queue_non_empty)
 
-lemma (in bfs_invar) head_queue_imp:
-  assumes "cond s"
-  shows
-    "Q_head (queue s) \<in> set (Q_list (queue s))"
-    "Q_head (queue s) \<notin> set (Q_list (queue (fold G src s)))"
-proof -
-  let ?u = "Q_head (queue s)"
-  show "?u \<in> set (Q_list (queue s))"
-    using queue_invar assms list_queue_non_empty
-    by (simp add: Q.list_head)
-  hence "?u \<notin> set (filter (Not \<circ> discovered src s) (G.out_neighborhood G (Q_head (queue s))))"
-    using gray_if_mem_queue
-    by fastforce
-  moreover have "?u \<notin> set (Q_list (Q_tail (queue s)))"
-    using queue_distinct
-    by (simp add: Q.list_queue[OF queue_invar list_queue_non_empty[OF assms]])
-  ultimately show "?u \<notin> set (Q_list (queue (fold G src s)))"
-    using assms
-    by (simp add: list_queue_fold_cong)
+lemma (in bfs_invar_not_DONE) head_queue_mem_queue:
+  shows "Q_head (queue s) \<in> set (Q_list (queue s))"
+  using invar_queue list_queue_non_empty
+  by (simp add: Q.list_head)
+
+lemma (in bfs_invar_not_DONE) not_white_head_queue:
+  shows "\<not> white s (Q_head (queue s))"
+  using head_queue_mem_queue
+  by (intro not_white_if_mem_queue)
+
+subsubsection \<open>\<close>
+
+lemma (in bfs_invar_not_DONE) follow_invar'_parent_fold:
+  shows "follow_invar' (P_lookup (parent (fold G src s)))"
+  unfolding follow_invar'_def T_fold_cong
+proof (rule wf_Un)
+  let ?r =
+    "{(Q_head (queue s), v) |v.
+      v \<in> set (G.adjacency G (Q_head (queue s))) \<and> \<not> discovered src (parent s) v}"
+  show "wf (T (parent s))"
+    using follow_invar'
+    by (simp add: follow_invar'_def)
+  have "\<not> white s (Q_head (queue s))"
+    using not_white_head_queue
+    .
+  thus "wf ?r"
+    by (simp add: wf_def)
+  show "Domain (T (parent s)) \<inter> Range ?r = {}"
+    using not_white_if_parent
+    by auto
 qed
 
-lemma (in bfs_invar) head_queue_if:
-  assumes "cond s"
+lemma (in bfs_invar_not_DONE) parent_fold:
+  shows "Tbd.parent (P_lookup (parent (fold G src s)))"
+proof (standard, goal_cases)
+  case 1
+  show ?case
+    by (intro follow_invar'_parent_fold)
+qed
+
+subsubsection \<open>@{thm bfs_invar.invar_queue}\<close>
+
+lemma (in bfs_invar_not_DONE) invar_queue_fold:
+  shows "Q_invar (queue (fold G src s))"
+  using invar_G invar_queue not_DONE
+  by (intro invar_queue_fold_2)
+
+subsubsection \<open>@{thm bfs_invar.invar_parent}\<close>
+
+lemma (in bfs_invar) invar_parent_fold:
+  shows "P_invar (parent (fold G src s))"
+  using invar_G invar_parent
+  by (intro invar_parent_fold_2)
+
+subsubsection \<open>@{thm bfs_invar.parent_src}\<close>
+
+lemma (in bfs_invar) parent_src_fold:
+  shows "P_lookup (parent (fold G src s)) src = None"
+  using invar_G invar_parent src_not_white
+  by (simp add: lookup_parent_fold_cong_2 parent_src)
+
+subsubsection \<open>Basic Lemmas\<close>
+
+lemma (in bfs_invar_not_DONE) head_queueI:
   assumes "v \<in> set (Q_list (queue s))"
   assumes "v \<notin> set (Q_list (queue (fold G src s)))"
   shows "v = Q_head (queue s)"
 proof -
   have "Q_list (queue s) = Q_head (queue s) # Q_list (Q_tail (queue s))"
-    using queue_invar assms(1)
-    by (intro list_queue_non_empty Q.list_queue)
+    using invar_queue list_queue_non_empty
+    by (intro Q.list_queue)
   thus ?thesis
     using assms
     by (simp add: list_queue_fold_cong)
 qed
 
-lemma (in bfs_invar) head_queue_iff:
-  assumes "cond s"
-  shows "v = Q_head (queue s) \<longleftrightarrow> v \<in> set (Q_list (queue s)) \<and> v \<notin> set (Q_list (queue (fold G src s)))"
-proof (standard, goal_cases)
-  case 1
-  show ?case
-    unfolding 1
-    using assms
-    by (intro head_queue_imp conjI)
-next
-  case 2
-  thus ?case
-    using assms
-    by (blast intro: head_queue_if)
-qed
+lemma (in bfs_invar) head_queueI_2:
+  assumes "P_lookup (parent s) v \<noteq> Some u"
+  assumes "P_lookup (parent (fold G src s)) v = Some u"
+  shows "u = Q_head (queue s)"
+  using assms
+  by (simp add: lookup_parent_fold_cong override_on_def split: if_splits(2))
+
+lemma (in bfs_invar_not_DONE) whiteD:
+  assumes "white s v"
+  shows "\<not> black (fold G src s) v"
+  using assms
+  by (auto simp add: discovered_def lookup_parent_fold_cong list_queue_fold_cong)
 
 lemma (in bfs_invar) not_white_imp_not_white_fold:
   assumes "\<not> white s v"
@@ -1354,198 +1224,17 @@ lemma (in bfs_invar) not_white_imp_not_white_fold:
   using assms
   by (auto simp add: discovered_def lookup_parent_fold_cong)
 
-lemma (in bfs_invar) white_not_white_fold_imp:
-  assumes "white s v"
-  assumes "\<not> white (fold G src s) v"
-  shows
-    "v \<in> set (G.out_neighborhood G (Q_head (queue s)))"
-    "P_lookup (parent (fold G src s)) v = Some (Q_head (queue s))"
-proof -
-  show "v \<in> set (G.out_neighborhood G (Q_head (queue s)))"
-    using assms G.out_neighborhood_finite
-    by (fastforce simp add: discovered_def lookup_parent_fold_cong)
-  thus "P_lookup (parent (fold G src s)) v = Some (Q_head (queue s))"
-    using assms G.out_neighborhood_finite
-    by (auto simp add: lookup_parent_fold_cong)
-qed
-
-subsubsection \<open>\<close>
-
-lemma (in bfs_invar) follow_invar'_parent_fold:
-  assumes "cond s"
-  shows "follow_invar' (P_lookup (parent (fold G src s)))"
-  unfolding follow_invar'_def T_fold_cong
-proof (rule wf_Un)
-  let ?r =
-    "{(Q_head (queue s), v) |v.
-      v \<in> set (G.out_neighborhood G (Q_head (queue s))) \<and> \<not> discovered src s v}"
-  show "wf (T s)"
-    using follow_invar'
-    by (simp add: follow_invar'_def)
-  have "gray s (Q_head (queue s))"
-    using assms
-    by (intro head_queue_imp(1) gray_if_mem_queue) simp+
-  thus "wf ?r"
-    by (simp add: wf_def)
-  show "Domain (T s) \<inter> Range ?r = {}"
-    using black_if_mem_ran
-    by (auto simp add: P.ran_def)
-qed
-
-lemma (in bfs_invar) parent_fold:
-  assumes "cond s"
-  shows "Tbd.parent (P_lookup (parent (fold G src s)))"
-  using assms
-  by unfold_locales (intro follow_invar'_parent_fold)
-
-subsubsection \<open>@{thm bfs_invar.queue_invar}\<close>
-
-lemma (in bfs_invar) queue_invar_fold:
-  assumes "cond s"
-  shows "Q_invar (queue (fold G src s))"
-  using G_invar queue_invar assms
-  by (intro queue_fold_invar_2)
-
-subsubsection \<open>@{thm bfs_invar.queue_distinct}\<close>
-
-lemma (in bfs_invar) queue_distinct_fold:
-  assumes "cond s"
-  shows "distinct (Q_list (queue (fold G src s)))"
-proof -
-  let ?l1 = "Q_list (Q_tail (queue s))"
-  let ?l2 = "filter (Not \<circ> discovered src s) (G.out_neighborhood G (Q_head (queue s)))"
-  have list_queue_non_empty: "Q_list (queue s) \<noteq> []"
-    using assms
-    by (intro list_queue_non_empty)
-  hence "\<And>v. v \<in> set ?l1 \<Longrightarrow> \<not> white s v"
-    using gray_if_mem_queue queue_invar
-    by (auto simp add: Q.list_tail intro: list.set_sel(2))
-  hence "set ?l1 \<inter> set ?l2 = {}"
-    by fastforce
-  moreover have "distinct ?l1"
-    using queue_distinct queue_invar list_queue_non_empty
-    by (auto simp add: Q.list_tail intro: distinct_tl)
-  moreover have "distinct ?l2"
-    using G_invar
-    by (intro G.out_neighborhood_distinct distinct_filter)
-  ultimately show ?thesis
-    using assms
-    by (simp add: list_queue_fold_cong)
-qed
-
-subsubsection \<open>@{thm bfs_invar.parent_invar}\<close>
-
-lemma (in bfs_invar) parent_invar_fold:
-  shows "P_invar (parent (fold G src s))"
-  using G_invar parent_invar
-  by (intro parent_fold_invar_2)
-
-subsubsection \<open>@{thm bfs_invar.parent_src}\<close>
-
-lemma (in bfs_invar) parent_src_fold:
-  shows "P_lookup (parent (fold G src s)) src = None"
-  using G_invar parent_invar src_not_white
-  by (simp add: lookup_parent_fold_cong_2 parent_src)
-
-subsubsection \<open>@{thm bfs_invar.gray_if_mem_queue}\<close>
-
-lemma (in bfs_invar) gray_if_mem_queue_fold:
-  assumes cond: "cond s"
-  assumes mem_queue_fold: "v \<in> set (Q_list (queue (fold G src s)))"
-  shows "gray (fold G src s) v"
-proof (cases "v \<in> set (Q_list (queue s))")
-  case True
-  hence "gray s v"
-    by (intro gray_if_mem_queue)
-  thus ?thesis
-    using cond not_white_imp_not_white_fold mem_queue_fold
-    by blast
-next
-  case False
-  have "Q_list (queue s) \<noteq> []"
-    using cond
-    by (intro list_queue_non_empty)
-  hence "v \<notin> set (Q_list (Q_tail (queue s)))"
-    using False queue_invar
-    by (auto simp add: Q.list_tail intro: list.set_sel(2))
-  hence "v \<in> set (G.out_neighborhood G (Q_head (queue s))) \<and> \<not> discovered src s v"
-    using mem_queue_fold cond
-    by (simp add: list_queue_fold_cong)
-  hence "\<not> white (fold G src s) v"
-    using assms(1)
-    by (fastforce simp add: discovered_def lookup_parent_fold_cong)
-  thus ?thesis
-    using mem_queue_fold
-    by blast
-qed
-
-subsubsection \<open>@{thm bfs_invar.black_if_mem_ran}\<close>
-
-lemma (in bfs_invar) head_queue_if_2:
-  assumes "v \<notin> P.ran (parent s)"
-  assumes "v \<in> P.ran (parent (fold G src s))"
-  shows "v = Q_head (queue s)"
-  using assms G_invar parent_invar
-  by (auto simp add: ran_parent_fold_cong split: if_splits(2))
-
-lemma (in bfs_invar) black_if_mem_ran_fold:
-  assumes cond: "cond s"
-  assumes mem_ran_fold: "v \<in> P.ran (parent (fold G src s))"
-  shows "black (fold G src s) v"
-proof (cases "v \<in> P.ran (parent s)")
-  case True
-  show ?thesis
-  proof (rule ccontr)
-    assume assm: "\<not> black (fold G src s) v"
-    have black: "black s v"
-      using True
-      by (intro black_if_mem_ran)
-    hence not_white_fold: "\<not> white (fold G src s) v"
-      by (intro black_imp_not_white not_white_imp_not_white_fold)
-    have "Q_list (queue s) \<noteq> []"
-      using cond
-      by (intro list_queue_non_empty)
-    hence "v \<notin> set (Q_list (Q_tail (queue s)))"
-      using black queue_invar
-      by (auto simp add: Q.list_tail intro: list.set_sel(2))
-    moreover have "v \<in> set (Q_list (queue (fold G src s)))"
-      using assm not_white_fold
-      by blast
-    ultimately have "white (fold G src s) v"
-      using cond black
-      by (simp add: discovered_def list_queue_fold_cong)
-    thus "False"
-      using not_white_fold
-      by blast
-  qed
-next
-  case False
-  have v_eq_Q_head_queue: "v = Q_head (queue s)"
-    using queue_invar False mem_ran_fold
-    by (intro head_queue_if_2)
-  then have "v \<in> set (Q_list (queue s))"
-    using cond
-    by (blast intro: head_queue_imp(1))
-  hence "\<not> white s v"
-    by (intro gray_if_mem_queue gray_imp_not_white)
-  hence "\<not> white (fold G src s) v"
-    by (intro not_white_imp_not_white_fold)
-  moreover have "v \<notin> set (Q_list (queue (fold G src s)))"
-    unfolding v_eq_Q_head_queue
-    using cond
-    by (intro head_queue_imp(2))
-  ultimately show ?thesis
-    by blast
-qed
-
-subsubsection \<open>@{thm bfs_invar.queue_sorted_wrt_dpath_length}\<close>
-
-lemma (in bfs_invar) not_white_imp_rev_follow_fold_eq_rev_follow:
-  assumes "cond s"
+lemma (in bfs_invar) not_white_imp_lookup_parent_fold_eq_lookup_parent:
   assumes "\<not> white s v"
-  shows "rev (parent.follow (P_lookup (parent (fold G src s))) v) = rev (follow v)"
+  shows "P_lookup (parent (fold G src s)) v = P_lookup (parent s) v"
   using assms
-proof (induct v rule: follow.pinduct[OF follow_dom])
+  by (simp add: lookup_parent_fold_cong)
+
+lemma (in bfs_invar_not_DONE) not_white_imp_rev_follow_fold_eq_rev_follow:
+  assumes "\<not> white s v"
+  shows "rev_follow (parent (fold G src s)) v = rev_follow (parent s) v"
+  using assms
+proof (induct v rule: follow_pinduct)
   case (1 v)
   show ?case
   proof (cases "v = src")
@@ -1556,8 +1245,8 @@ proof (induct v rule: follow.pinduct[OF follow_dom])
       using parent_src parent_src_fold
       by simp+
     hence
-      "rev (follow v) = [v]"
-      "rev (parent.follow (P_lookup (parent (fold G src s))) v) = [v]"
+      "rev_follow (parent s) v = [v]"
+      "rev_follow (parent (fold G src s)) v = [v]"
       using "1.prems"(1) parent_fold
       by (simp_all add: follow_psimps parent.follow_psimps)
     thus ?thesis
@@ -1567,590 +1256,786 @@ proof (induct v rule: follow.pinduct[OF follow_dom])
     then obtain u where u:
       "P_lookup (parent s) v = Some u"
       "\<not> white s u"
-      using False "1.prems"(2) black_if_mem_ran
-      by (auto simp add: discovered_def P.ran_def)
+      using "1.prems"(1) not_white_if_parent
+      by (auto simp add: discovered_def)
     moreover hence "P_lookup (parent (fold G src s)) v = Some u"
-      using "1.prems"(2)
-      by (simp add: lookup_parent_fold_cong map_add_Some_iff)
+      using "1.prems"
+      by (simp add: not_white_imp_lookup_parent_fold_eq_lookup_parent)
     ultimately have
-      "rev (follow v) = rev (follow u) @ [v]"
-      "rev (parent.follow (P_lookup (parent (fold G src s))) v) =
-       rev (parent.follow (P_lookup (parent (fold G src s))) u) @ [v]"
+      "rev_follow (parent s) v = rev_follow (parent s) u @ [v]"
+      "rev_follow (parent (fold G src s)) v = rev_follow (parent (fold G src s)) u @ [v]"
       using "1.prems"(1) parent_fold
       by (simp_all add: follow_psimps parent.follow_psimps)
     thus ?thesis
-      using u "1.prems"(1)
+      using u
       by (simp add: "1.hyps"(2))
   qed
 qed
 
-lemma (in bfs_invar) mem_filter_imp_dpath_length:
-  assumes "cond s"
-  assumes "v \<in> set (filter (Not \<circ> discovered src s) (G.out_neighborhood G (Q_head (queue s))))"
+lemmas (in bfs_invar_not_DONE) not_whiteD =
+  not_white_imp_not_white_fold
+  not_white_imp_lookup_parent_fold_eq_lookup_parent
+  not_white_imp_rev_follow_fold_eq_rev_follow
+
+lemma (in bfs_invar_not_DONE) mem_filterD:
+  assumes "v \<in> set (filter (Not \<circ> discovered src (parent s)) (G.adjacency G (Q_head (queue s))))"
   shows
-    "dpath_length (rev (parent.follow (P_lookup (parent (fold G src s))) v)) =
-     dpath_length (rev (parent.follow (P_lookup (parent (fold G src s))) (Q_head (queue s)))) + 1"
-    "dpath_length (rev (parent.follow (P_lookup (parent (fold G src s))) (last (Q_list (queue s))))) \<le>
-     dpath_length (rev (parent.follow (P_lookup (parent (fold G src s))) v))"
+    "d (parent (fold G src s)) v = d (parent (fold G src s)) (Q_head (queue s)) + 1"
+    "d (parent (fold G src s)) (last (Q_list (queue s))) \<le> d (parent (fold G src s)) v"
 proof -
   let ?u = "Q_head (queue s)"
   have "P_lookup (parent (fold G src s)) v = Some ?u"
     using assms
     by (simp add: lookup_parent_fold_cong)
-  hence
-    "rev (parent.follow (P_lookup (parent (fold G src s))) v) =
-     rev (parent.follow (P_lookup (parent (fold G src s))) ?u) @ [v]"
+  hence "rev_follow (parent (fold G src s)) v = rev_follow (parent (fold G src s)) ?u @ [v]"
     using assms(1) parent_fold
     by (simp add: parent.follow_psimps)
-  thus dpath_length_eq:
-    "dpath_length (rev (parent.follow (P_lookup (parent (fold G src s))) v)) =
-     dpath_length (rev (parent.follow (P_lookup (parent (fold G src s))) (Q_head (queue s)))) + 1"
+  thus d_eq: "d (parent (fold G src s)) v = d (parent (fold G src s)) (Q_head (queue s)) + 1"
     using assms(1) parent_fold parent.follow_non_empty
     by (fastforce simp add: dpath_length_snoc)
 
-  have
-    "dpath_length (rev (parent.follow (P_lookup (parent (fold G src s))) (last (Q_list (queue s))))) =
-     dpath_length (rev (follow (last (Q_list (queue s)))))"
-    using assms list_queue_non_empty gray_if_mem_queue
-    by (simp add: not_white_imp_rev_follow_fold_eq_rev_follow)
-  also have "... \<le> dpath_length (rev (follow ?u)) + 1"
-    using assms tbd_dpath_length
-    by (simp add: cond_def)
-  also have "... = dpath_length (rev (parent.follow (P_lookup (parent (fold G src s))) ?u)) + 1"
-    using assms head_queue_imp(1) gray_if_mem_queue
-    by (simp add: not_white_imp_rev_follow_fold_eq_rev_follow)
-  also have "... = dpath_length (rev (parent.follow (P_lookup (parent (fold G src s))) v))"
-    unfolding dpath_length_eq
+  have "d (parent (fold G src s)) (last (Q_list (queue s))) = d (parent s) (last (Q_list (queue s)))"
+    using assms list_queue_non_empty not_white_if_mem_queue
+    by (simp add: not_whiteD(3))
+  also have "... \<le> d (parent s) ?u + 1"
+    using not_DONE d_last_queue_le
+    by (simp add: DONE_def)
+  also have "... = d (parent (fold G src s)) ?u + 1"
+    using assms not_white_head_queue
+    by (simp add: not_whiteD(3))
+  also have "... = d (parent (fold G src s)) v"
+    unfolding d_eq
     ..
-  finally show
-    "dpath_length (rev (parent.follow (P_lookup (parent (fold G src s))) (last (Q_list (queue s))))) \<le>
-     dpath_length (rev (parent.follow (P_lookup (parent (fold G src s))) v))"
+  finally show "d (parent (fold G src s)) (last (Q_list (queue s))) \<le> d (parent (fold G src s)) v"
     .
 qed
 
-lemma (in bfs_invar) queue_sorted_wrt_dpath_length_fold_aux:
-  assumes cond: "cond s"
-  assumes u_mem_Q_tail_queue: "u \<in> set (Q_list (Q_tail (queue s)))"
-  assumes v_mem_filter:
-    "v \<in> set (filter (Not \<circ> discovered src s) (G.out_neighborhood G (Q_head (queue s))))"
+lemma (in bfs_invar) white_not_white_foldD:
+  assumes "white s v"
+  assumes "\<not> white (fold G src s) v"
   shows
-    "dpath_length (rev (parent.follow (P_lookup (parent (fold G src s))) u)) \<le>
-     dpath_length (rev (parent.follow (P_lookup (parent (fold G src s))) v))"
+    "v \<in> set (G.adjacency G (Q_head (queue s)))"
+    "P_lookup (parent (fold G src s)) v = Some (Q_head (queue s))"
+proof -
+  show "v \<in> set (G.adjacency G (Q_head (queue s)))"
+    using assms
+    by (fastforce simp add: discovered_def lookup_parent_fold_cong)
+  thus "P_lookup (parent (fold G src s)) v = Some (Q_head (queue s))"
+    using assms
+    by (auto simp add: lookup_parent_fold_cong)
+qed
+
+lemma (in bfs_invar_not_DONE) white_not_white_foldD_2:
+  assumes "white s v"
+  assumes "\<not> white (fold G src s) v"
+  shows "d (parent (fold G src s)) v = d (parent (fold G src s)) (Q_head (queue s)) + 1"
+  using parent_fold assms
+  by (fastforce intro: white_not_white_foldD(2) parent_imp_d)
+
+lemmas (in bfs_invar_not_DONE) white_not_white_foldD =
+  white_not_white_foldD
+  white_not_white_foldD_2
+
+subsubsection \<open>@{thm bfs_invar.parent_imp_edge}\<close>
+
+lemma (in bfs_invar_not_DONE) parent_imp_edge_fold:
+  assumes "P_lookup (parent (fold G src s)) v = Some u"
+  shows "(u, v) \<in> G.dE G"
+proof (cases "P_lookup (parent s) v = Some u")
+  case True
+  thus ?thesis
+    by (intro parent_imp_edge)
+next
+  case False
+  thus ?thesis
+    using assms head_queueI_2 G.mem_adjacency_iff_edge
+    by (fastforce simp add: lookup_parent_fold_cong)
+qed
+
+subsubsection \<open>@{thm bfs_invar.not_white_if_mem_queue}\<close>
+
+lemma (in bfs_invar_not_DONE) not_white_if_mem_queue_fold:
+  assumes "v \<in> set (Q_list (queue (fold G src s)))"
+  shows "\<not> white (fold G src s) v"
+proof (cases "v \<in> set (Q_list (queue s))")
+  case True
+  thus ?thesis
+    by (intro not_white_if_mem_queue not_whiteD(1))
+next
+  case False
+  hence "v \<notin> set (Q_list (Q_tail (queue s)))"
+    using invar_queue list_queue_non_empty
+    by (auto simp add: Q.list_tail intro: list.set_sel(2))
+  hence "v \<in> set (G.adjacency G (Q_head (queue s))) \<and> \<not> discovered src (parent s) v"
+    using assms
+    by (simp add: list_queue_fold_cong)
+  thus ?thesis
+    using assms
+    by (fastforce simp add: discovered_def lookup_parent_fold_cong)
+qed
+
+subsubsection \<open>@{thm bfs_invar.not_white_if_parent}\<close>
+
+lemma (in bfs_invar_not_DONE) not_white_if_parent_fold:
+  assumes "P_lookup (parent (fold G src s)) v = Some u"
+  shows "\<not> white (fold G src s) u"
+proof (cases "P_lookup (parent s) v = Some u")
+  case True
+  thus ?thesis
+    by (intro not_white_if_parent not_whiteD(1))
+next
+  case False
+  hence "u = Q_head (queue s)"
+    using assms
+    by (intro head_queueI_2)
+  thus ?thesis
+    using not_white_head_queue
+    by (intro not_whiteD(1)) simp
+qed
+
+subsubsection \<open>@{thm bfs_invar.black_imp_adjacency_not_white}\<close>
+
+lemma (in bfs_invar_not_DONE) black_imp_adjacency_not_white_fold:
+  assumes "black (fold G src s) u"
+  assumes "(u, v) \<in> G.dE G"
+  shows "\<not> white (fold G src s) v"
+proof (induct s u rule: vertex_color_induct)
+  case white
+  thus ?case
+    using assms(1) whiteD
+    by blast
+next
+  case gray
+  hence "u = Q_head (queue s)"
+    using assms(1)
+    by (intro head_queueI) simp+
+  thus ?case
+    using assms(2)
+    by (simp add: discovered_def lookup_parent_fold_cong override_on_def G.mem_adjacency_iff_edge)
+next
+  case black
+  thus ?case
+    using assms(2)
+    by (intro black_imp_adjacency_not_white not_whiteD(1))
+qed
+
+subsubsection \<open>@{thm bfs_invar.queue_sorted_wrt_d}\<close>
+
+lemma (in bfs_invar_not_DONE) queue_sorted_wrt_d_fold_aux:
+  assumes u_mem_tail_queue: "u \<in> set (Q_list (Q_tail (queue s)))"
+  assumes v_mem_filter: "v \<in> set (filter (Not \<circ> discovered src (parent s)) (G.adjacency G (Q_head (queue s))))"
+  shows "d (parent (fold G src s)) u \<le> d (parent (fold G src s)) v"
 proof -
   have u_mem_queue: "u \<in> set (Q_list (queue s))"
-    using u_mem_Q_tail_queue queue_invar cond list_queue_non_empty
+    using u_mem_tail_queue invar_queue list_queue_non_empty
     by (auto simp add: Q.list_tail intro: list.set_sel(2))
-  have
-    "dpath_length (rev (parent.follow (P_lookup (parent (fold G src s))) u)) =
-     dpath_length (rev (follow u))"
-    using cond u_mem_queue gray_if_mem_queue
-    by (simp add: not_white_imp_rev_follow_fold_eq_rev_follow)
-  also have "... \<le> dpath_length (rev (follow (last (Q_list (queue s)))))"
+  have "d (parent (fold G src s)) u = d (parent s) u"
+    using u_mem_queue not_white_if_mem_queue
+    by (simp add: not_whiteD(3))
+  also have "... \<le> d (parent s) (last (Q_list (queue s)))"
     using u_mem_queue
-    by (intro mem_queue_imp_dpath_length_last_queue)
-  also have "... = dpath_length (rev (parent.follow (P_lookup (parent (fold G src s))) (last (Q_list (queue s)))))"
-    using cond list_queue_non_empty gray_if_mem_queue
-    by (simp add: not_white_imp_rev_follow_fold_eq_rev_follow)
-  also have "... \<le> dpath_length (rev (parent.follow (P_lookup (parent (fold G src s))) v))"
-    using cond v_mem_filter
-    by (intro mem_filter_imp_dpath_length(2))
+    by (intro mem_queue_imp_d_le)
+  also have "... = d (parent (fold G src s)) (last (Q_list (queue s)))"
+    using list_queue_non_empty not_white_if_mem_queue
+    by (simp add: not_whiteD(3))
+  also have "... \<le> d (parent (fold G src s)) v"
+    using v_mem_filter
+    by (intro mem_filterD(2))
   finally show ?thesis
     .
 qed
 
-lemma (in bfs_invar) tbd_dpath_length_fold_aux:
-  assumes cond: "cond s"
+lemma (in bfs_invar_not_DONE) queue_sorted_wrt_d_fold:
+  shows "sorted_wrt (\<lambda>u v. d (parent (fold G src s)) u \<le> d (parent (fold G src s)) v) (Q_list (queue (fold G src s)))"
+proof -
+  let ?P = "\<lambda>u v. d (parent (fold G src s)) u \<le> d (parent (fold G src s)) v"
+  have "sorted_wrt ?P (Q_list (queue s))"
+    using queue_sorted_wrt_d not_white_if_mem_queue sorted_wrt_mono_rel[of "(Q_list (queue s))"]
+    by (simp add: not_whiteD(3))
+  hence "sorted_wrt ?P (Q_list (Q_tail (queue s)))"
+    by (simp add: Q.list_queue[OF invar_queue list_queue_non_empty])
+  moreover have "sorted_wrt ?P (filter (Not \<circ> discovered src (parent s)) (G.adjacency G (Q_head (queue s))))"
+    by (auto simp add: mem_filterD(1) intro: sorted_wrt_if)
+  moreover have
+    "\<forall>u\<in>set (Q_list (Q_tail (queue s))).
+      \<forall>v\<in>set (filter (Not \<circ> discovered src (parent s)) (G.adjacency G (Q_head (queue s)))).
+       d (parent (fold G src s)) u \<le> d (parent (fold G src s)) v"
+    by (blast intro: queue_sorted_wrt_d_fold_aux)
+  ultimately show ?thesis 
+    by (simp add: list_queue_fold_cong sorted_wrt_append)
+qed
+
+subsubsection \<open>@{thm bfs_invar.d_last_queue_le}\<close>
+
+lemma (in bfs_invar_not_DONE) d_last_queue_le_fold_aux:
   assumes "\<not> Q_is_empty (queue (fold G src s))"
-  shows
-    "dpath_length (rev (parent.follow (P_lookup (parent (fold G src s))) (last (Q_list (queue (fold G src s)))))) \<le>
-     dpath_length (rev (parent.follow (P_lookup (parent (fold G src s))) (Q_head (queue s)))) + 1"
-proof (cases "filter (Not \<circ> discovered src s) (G.out_neighborhood G (Q_head (queue s))) = []")
+  shows "d (parent (fold G src s)) (last (Q_list (queue (fold G src s)))) \<le> d (parent (fold G src s)) (Q_head (queue s)) + 1"
+proof (cases "filter (Not \<circ> discovered src (parent s)) (G.adjacency G (Q_head (queue s))) = []")
   case True
   hence list_tail_non_empty: "Q_list (Q_tail (queue s)) \<noteq> []"
-    using assms G_invar queue_invar queue_fold_invar_2
+    using invar_G invar_queue not_DONE invar_queue_fold_2 assms
     by (simp add: list_queue_fold_cong Q.is_empty)
 
   hence "last (Q_list (queue (fold G src s))) = last (Q_list (Q_tail (queue s)))"
-    unfolding list_queue_fold_cong[OF cond] last_appendL[OF True]
+    unfolding list_queue_fold_cong last_appendL[OF True]
     by blast
   hence "last (Q_list (queue (fold G src s))) = last (Q_list (queue s))"
     using list_tail_non_empty
-    by (simp add: Q.list_queue[OF queue_invar list_queue_non_empty[OF assms(1)]])
-  hence
-    "dpath_length (rev (parent.follow (P_lookup (parent (fold G src s))) (last (Q_list (queue (fold G src s)))))) =
-     dpath_length (rev (follow (last (Q_list (queue s)))))"
-    using cond list_queue_non_empty gray_if_mem_queue
-    by (simp add: not_white_imp_rev_follow_fold_eq_rev_follow)
-  also have "... \<le> dpath_length (rev (follow (Q_head (queue s)))) + 1"
-    using queue_invar cond list_queue_non_empty tbd_dpath_length
+    by (simp add: Q.list_queue[OF invar_queue list_queue_non_empty])
+  hence "d (parent (fold G src s)) (last (Q_list (queue (fold G src s)))) = d (parent s) (last (Q_list (queue s)))"
+    using list_queue_non_empty not_white_if_mem_queue
+    by (simp add: not_whiteD(3))
+  also have "... \<le> d (parent s) (Q_head (queue s)) + 1"
+    using invar_queue list_queue_non_empty d_last_queue_le
     by (simp add: Q.is_empty)
-  also have "... = dpath_length (rev (parent.follow (P_lookup (parent (fold G src s))) (Q_head (queue s)))) + 1"
-    using cond head_queue_imp(1) gray_if_mem_queue
-    by (simp add: not_white_imp_rev_follow_fold_eq_rev_follow)
+  also have "... = d (parent (fold G src s)) (Q_head (queue s)) + 1"
+    using not_white_head_queue
+    by (simp add: not_whiteD(3))
   finally show ?thesis
     .
 next
   case False
   hence
     "last (Q_list (queue (fold G src s))) \<in>
-     set (filter (Not \<circ> discovered src s) (G.out_neighborhood G (Q_head (queue s))))"
-    unfolding list_queue_fold_cong[OF cond] last_appendR[OF False]
+     set (filter (Not \<circ> discovered src (parent s)) (G.adjacency G (Q_head (queue s))))"
+    unfolding list_queue_fold_cong last_appendR[OF False]
     by (intro last_in_set)
-  with cond
-  show ?thesis
-    by (simp add: mem_filter_imp_dpath_length(1))
+  thus ?thesis
+    by (simp add: mem_filterD(1))
 qed
 
-lemma (in bfs_invar) tbd_dpath_length_fold_aux_2:
-  assumes cond: "cond s"
+lemma (in bfs_invar_not_DONE) d_last_queue_le_fold_aux_2:
   assumes "\<not> Q_is_empty (queue (fold G src s))"
-  shows
-    "dpath_length (rev (parent.follow (P_lookup (parent (fold G src s))) (Q_head (queue s)))) \<le>
-     dpath_length (rev (parent.follow (P_lookup (parent (fold G src s))) (Q_head (queue (fold G src s)))))"
+  shows "d (parent (fold G src s)) (Q_head (queue s)) \<le> d (parent (fold G src s)) (Q_head (queue (fold G src s)))"
 proof (cases "Q_list (Q_tail (queue s)) = []")
   case True
   have "Q_head (queue (fold G src s)) = hd (Q_list (queue (fold G src s)))"
-    using assms G_invar queue_invar queue_fold_invar_2
+    using invar_G invar_queue not_DONE invar_queue_fold_2 assms
     by (simp add: Q.is_empty Q.list_head)
   hence
     "Q_head (queue (fold G src s)) =
-     hd (filter (Not \<circ> discovered src s) (G.out_neighborhood G (Q_head (queue s))))"
-    using cond True
-    by (simp add: list_queue_fold_cong)
-  moreover have
-    "filter (Not \<circ> discovered src s) (G.out_neighborhood G (Q_head (queue s))) \<noteq> []"
-    using assms G_invar queue_invar queue_fold_invar_2 True
-    by (simp add: Q.is_empty list_queue_fold_cong)
-  ultimately have Q_head_queue_fold_mem_filter:
+     hd (filter (Not \<circ> discovered src (parent s)) (G.adjacency G (Q_head (queue s))))"
+    by (simp add: True list_queue_fold_cong)
+  moreover have "filter (Not \<circ> discovered src (parent s)) (G.adjacency G (Q_head (queue s))) \<noteq> []"
+    using invar_G invar_queue not_DONE invar_queue_fold_2 assms
+    by (simp add: True Q.is_empty list_queue_fold_cong)
+  ultimately have head_queue_fold_mem_filter:
     "Q_head (queue (fold G src s)) \<in>
-     set (filter (Not \<circ> discovered src s) (G.out_neighborhood G (Q_head (queue s))))"
+     set (filter (Not \<circ> discovered src (parent s)) (G.adjacency G (Q_head (queue s))))"
     using list.set_sel(1)
     by metis
 
-  have
-    "dpath_length (rev (parent.follow (P_lookup (parent (fold G src s))) (Q_head (queue s)))) =
-     dpath_length (rev (follow (Q_head (queue s))))"
-    using cond head_queue_imp(1) gray_if_mem_queue
-    by (simp add: not_white_imp_rev_follow_fold_eq_rev_follow)
-  also have "... \<le> dpath_length (rev (follow (last (Q_list (queue s)))))"
-    using cond
-    by (intro head_queue_imp(1) mem_queue_imp_dpath_length_last_queue)
-  also have
-    "... = dpath_length (rev (parent.follow (P_lookup (parent (fold G src s))) (last (Q_list (queue s)))))"
-    using cond list_queue_non_empty gray_if_mem_queue
-    by (simp add: not_white_imp_rev_follow_fold_eq_rev_follow)
-  also have "... \<le> dpath_length (rev (parent.follow (P_lookup (parent (fold G src s))) (Q_head (queue (fold G src s)))))"
-    using cond Q_head_queue_fold_mem_filter
-    by (intro mem_filter_imp_dpath_length(2))
+  have "d (parent (fold G src s)) (Q_head (queue s)) = d (parent s) (Q_head (queue s))"
+    using not_white_head_queue
+    by (simp add: not_whiteD(3))
+  also have "... \<le> d (parent s) (last (Q_list (queue s)))"
+    by (intro head_queue_mem_queue mem_queue_imp_d_le)
+  also have "... = d (parent (fold G src s)) (last (Q_list (queue s)))"
+    using list_queue_non_empty not_white_if_mem_queue
+    by (simp add: not_whiteD(3))
+  also have "... \<le> d (parent (fold G src s)) (Q_head (queue (fold G src s)))"
+    using head_queue_fold_mem_filter
+    by (intro mem_filterD(2))
   finally show ?thesis
     .
 next
   case False
   have "Q_head (queue (fold G src s)) = hd (Q_list (queue (fold G src s)))"
-    using assms G_invar queue_invar queue_fold_invar_2
+    using invar_G invar_queue not_DONE invar_queue_fold_2 assms
     by (simp add: Q.is_empty Q.list_head)
   hence "Q_head (queue (fold G src s)) = hd (Q_list (Q_tail (queue s)))"
-    using cond False
+    using False
     by (simp add: list_queue_fold_cong)
-  hence Q_head_queue_fold_mem_list_queue: "Q_head (queue (fold G src s)) \<in> set (Q_list (queue s))"
-    using False queue_invar cond list_queue_non_empty
+  hence head_queue_fold_mem_queue: "Q_head (queue (fold G src s)) \<in> set (Q_list (queue s))"
+    using False invar_queue list_queue_non_empty
     by (auto simp add: Q.list_tail intro: list.set_sel(2))
 
-  have
-    "dpath_length (rev (parent.follow (P_lookup (parent (fold G src s))) (Q_head (queue s)))) =
-     dpath_length (rev (follow (Q_head (queue s))))"
-    using cond head_queue_imp(1) gray_if_mem_queue
-    by (simp add: not_white_imp_rev_follow_fold_eq_rev_follow)
-  also have "... \<le> dpath_length (rev (follow (Q_head (queue (fold G src s)))))"
-    using Q_head_queue_fold_mem_list_queue
-    by (intro mem_queue_imp_dpath_length_head_queue)
-  also have "... = dpath_length (rev (parent.follow (P_lookup (parent (fold G src s))) (Q_head (queue (fold G src s)))))"
-    using cond Q_head_queue_fold_mem_list_queue gray_if_mem_queue
-    by (simp add: not_white_imp_rev_follow_fold_eq_rev_follow)
+  have "d (parent (fold G src s)) (Q_head (queue s)) = d (parent s) (Q_head (queue s))"
+    using not_white_head_queue
+    by (simp add: not_whiteD(3))
+  also have "... \<le> d (parent s) (Q_head (queue (fold G src s)))"
+    using head_queue_fold_mem_queue
+    by (intro mem_queue_imp_d_ge)
+  also have "... = d (parent (fold G src s)) (Q_head (queue (fold G src s)))"
+    using head_queue_fold_mem_queue not_white_if_mem_queue
+    by (simp add: not_whiteD(3))
   finally show ?thesis
     .
 qed
 
-lemma (in bfs_invar) queue_sorted_wrt_dpath_length_fold:
-  assumes "cond s"
-  shows
-    "sorted_wrt
-      (\<lambda>u v. dpath_length (rev (parent.follow (P_lookup (parent (fold G src s))) u)) \<le>
-             dpath_length (rev (parent.follow (P_lookup (parent (fold G src s))) v)))
-      (Q_list (queue (fold G src s)))"
-proof -
-  let ?P =
-    "\<lambda>u v. dpath_length (rev (parent.follow (P_lookup (parent (fold G src s))) u)) \<le>
-           dpath_length (rev (parent.follow (P_lookup (parent (fold G src s))) v))"
-  have list_queue_non_empty: "Q_list (queue s) \<noteq> []"
-    using assms
-    by (intro list_queue_non_empty)
-  hence
-    "sorted_wrt
-      (\<lambda>u v. dpath_length (rev (follow u)) \<le> dpath_length (rev (follow v)))
-      (Q_list (queue s))"
-    using queue_invar queue_sorted_wrt_dpath_length
-    by (simp add: Q.is_empty)
-  hence "sorted_wrt ?P (Q_list (queue s))"
-    using assms gray_if_mem_queue sorted_wrt_mono_rel[of "(Q_list (queue s))"]
-    by (simp add: not_white_imp_rev_follow_fold_eq_rev_follow)
-  hence "sorted_wrt ?P (Q_list (Q_tail (queue s)))"
-    by (simp add: Q.list_queue[OF queue_invar list_queue_non_empty])
-  moreover have
-    "sorted_wrt
-      ?P
-      (filter (Not \<circ> discovered src s) (G.out_neighborhood G (Q_head (queue s))))"
-    using assms
-    by (auto simp add: mem_filter_imp_dpath_length(1) intro: sorted_wrt_if)
-  moreover have
-    "\<forall>u\<in>set (Q_list (Q_tail (queue s))).
-      \<forall>v\<in>set (filter (Not \<circ> discovered src s) (G.out_neighborhood G (Q_head (queue s)))).
-       dpath_length (rev (parent.follow (P_lookup (parent (fold G src s))) u)) \<le>
-       dpath_length (rev (parent.follow (P_lookup (parent (fold G src s))) v))"
-    using assms
-    by (blast intro: queue_sorted_wrt_dpath_length_fold_aux)
-  ultimately show ?thesis 
-    using assms
-    by (simp add: list_queue_fold_cong sorted_wrt_append)
-qed
-
-lemma (in bfs_invar) tbd_dpath_length_fold:
-  assumes "cond s"
+lemma (in bfs_invar_not_DONE) d_last_queue_le_fold:
   assumes "\<not> Q_is_empty (queue (fold G src s))"
-  shows
-    "dpath_length (rev (parent.follow (P_lookup (parent (fold G src s))) (last (Q_list (queue (fold G src s)))))) \<le>
-     dpath_length (rev (parent.follow (P_lookup (parent (fold G src s))) (Q_head (queue (fold G src s))))) + 1"
+  shows "d (parent (fold G src s)) (last (Q_list (queue (fold G src s)))) \<le> d (parent (fold G src s)) (Q_head (queue (fold G src s))) + 1"
 proof -
-  have
-    "dpath_length (rev (parent.follow (P_lookup (parent (fold G src s))) (last (Q_list (queue (fold G src s)))))) \<le>
-     dpath_length (rev (parent.follow (P_lookup (parent (fold G src s))) (Q_head (queue s)))) + 1"
+  have "d (parent (fold G src s)) (last (Q_list (queue (fold G src s)))) \<le> d (parent (fold G src s)) (Q_head (queue s)) + 1"
     using assms
-    by (intro tbd_dpath_length_fold_aux)
-  also have "... \<le> dpath_length (rev (parent.follow (P_lookup (parent (fold G src s))) (Q_head (queue (fold G src s))))) + 1"
+    by (intro d_last_queue_le_fold_aux)
+  also have "... \<le> d (parent (fold G src s)) (Q_head (queue (fold G src s))) + 1"
     using assms
-    by (auto intro: tbd_dpath_length_fold_aux_2)
+    by (auto intro: d_last_queue_le_fold_aux_2)
   finally show ?thesis
     .
 qed
 
-subsubsection \<open>@{thm bfs_invar.not_white_imp_shortest_dpath}\<close>
+subsubsection \<open>@{thm bfs_invar.d_triangle_inequality}\<close>
 
-lemma (in bfs_invar) not_white_imp_shortest_dpath_fold_case_1_subcase_3_aux:
-  assumes cond: "cond s"
-  assumes dist_less: "dist G src v < dist G src (Q_head (queue s)) + 1"
-  assumes dpath_bet: "dpath_bet (G.E G) (l @ [u, u']) src v"
-  assumes dpath_length: "dpath_length (l @ [u, u']) = dist G src v"
-  assumes white: "white s v"
-  shows "False"
-proof -
-  let ?u = "Q_head (queue s)"
-  have "dist G src u + 1 = dist G src v"
-    using E_finite dpath_bet dpath_length
-    by (auto intro: shortest_dpathE_2)
-  hence "dist G src u + 1 < dist G src ?u + 1"
-    using dist_less
-    by simp
-  hence "dist G src u < dist G src ?u"
-    unfolding plus_1_eSuc(2) eSuc_mono
-    .
-  thus ?thesis
-  proof (induct s u rule: vertex_color_induct)
-    case white
-    have "dist G src ?u \<le> dist G src (last (Q_list (queue s)))"
-      using cond list_queue_non_empty
-      by (intro mem_queue_imp_dist_head_queue) simp
-    also have "... \<le> dist G src u"
-      using white.hyps cond white_imp_dist_ge
-      by (simp add: cond_def)
-    finally show ?case
-      using white.prems
-      by simp
-  next
-    case gray
-    hence "dist G src ?u \<le> dist G src u"
-      by (intro mem_queue_imp_dist_head_queue) simp
-    thus ?case
-      using gray.prems
-      by simp
-  next
-    case black
-    hence "v \<in> set (G.out_neighborhood G u)"
-      using dpath_bet
-      by (auto simp add: dpath_bet_def G.mem_out_neighborhood_iff_edge intro: dpath_snoc_edge_2)
-    hence "\<not> white s v"
-      using black.hyps black_imp_out_neighborhood_not_white
-      by blast
-    thus ?case
-      using white
-      by simp
-  qed
-qed
-
-lemma (in bfs_invar) not_white_imp_shortest_dpath_fold_case_1_aux:
-  assumes cond: "cond s"
-  assumes white: "white s v"
-  assumes reachable: "reachable (G.E G) src v"
-  assumes v_mem_out_neighborhood: "v \<in> set (G.out_neighborhood G (Q_head (queue s)))"
-  shows "dist G src (Q_head (queue s)) + 1 = dist G src v"
-proof (rule antisym, rule ccontr, goal_cases)
+lemma (in bfs_invar) white_imp_gray_ancestor:
+  assumes "dpath_bet (G.dE G) p u w"
+  assumes "\<not> white s u"
+  assumes "white s w"
+  obtains v where
+    "v \<in> set p"
+    "gray s v"
+  using assms
+proof (induct p arbitrary: w rule: dpath_rev_induct)
   case 1
-  let ?u = "Q_head (queue s)"
-  assume "\<not> dist G src ?u + 1 \<le> dist G src v"
-  hence "dist G src v < dist G src ?u + 1"
-    by fastforce
-  moreover obtain p where
-    "dpath_bet (G.E G) p src v"
-    "dpath_length p = dist G src v"
-    using E_finite reachable
-    by (elim dist_dpath_betE)
-  ultimately show ?case
-    using white
-  proof (induct p arbitrary: v rule: dpath_rev_induct)
-    case 1
-    thus ?case
-      by auto
-  next
-    case (2 u)
-    hence "[u] = [src] \<and> src = v"
-      by (intro hd_of_dpath_bet' last_of_dpath_bet list_length_1) simp
-    hence "white s src"
-      using "2.prems"(4)
-      by simp
-    thus ?case
-      by (simp add: discovered_def)
-  next
-    case (3 u u' l)
-    with cond
-    show ?case
-      by (intro not_white_imp_shortest_dpath_fold_case_1_subcase_3_aux)
-  qed
+  thus ?case
+    by simp
 next
   case 2
+  thus ?case
+    using hd_of_dpath_bet' last_of_dpath_bet
+    by (fastforce intro: list_length_1)
+next
+  case (3 v v' l)
   show ?case
-    using cond head_queue_mem_V v_mem_out_neighborhood E_finite dist_triangle_inequality_edge
-    by (simp add: G.mem_out_neighborhood_iff_edge)
+  proof (induct s v rule: vertex_color_induct)
+    case white
+    have "dpath_bet (G.dE G) (l @ [v]) u v"
+      using "3.prems"(2)
+      by (intro dpath_bet_pref) simp
+    with "3.prems"(1)
+    show ?case
+      using "3.prems"(3) white
+      by (force intro: "3.hyps")
+  next
+    case gray
+    thus ?case
+      by (auto intro: "3.prems"(1))
+  next
+    case black
+    have "(v, w) \<in> G.dE G"
+      using "3.prems"(2)
+      by (auto simp add: dpath_bet_def intro: dpath_snoc_edge_2)
+    thus ?case
+      using black black_imp_adjacency_not_white "3.prems"(4)
+      by blast
+  qed
 qed
 
-lemma (in bfs_invar) not_white_imp_shortest_dpath_fold:
-  assumes cond: "cond s"
-  assumes not_white_fold: "\<not> white (fold G src s) v"
-  shows "is_shortest_dpath G (rev (parent.follow (P_lookup (parent (fold G src s))) v)) src v"
-proof (cases "white s v", standard)
-  let ?u = "Q_head (queue s)"
-  case True
-  hence
-    v_mem_out_neighborhood: "v \<in> set (G.out_neighborhood G ?u)" and
-    parent_fold_v_eq_head_queue: "P_lookup (parent (fold G src s)) v = Some ?u"
-    using assms
-    by (auto intro: white_not_white_fold_imp)
-  have Q_head_queue_not_white: "\<not> white s ?u"
-    using cond
-    by (intro head_queue_imp(1) gray_if_mem_queue gray_imp_not_white)
-  hence rev_follow_head_queue_shortest_dpath: "is_shortest_dpath G (rev (follow ?u)) src ?u"
-    by (intro not_white_imp_shortest_dpath)
-  have
-    "rev (parent.follow (P_lookup (parent (fold G src s))) v) =
-     rev (parent.follow (P_lookup (parent (fold G src s))) ?u) @ [v]"
-    using cond parent_fold
-    by (simp add: parent.follow_psimps parent_fold_v_eq_head_queue)
-  hence rev_follow_fold_eq: "rev (parent.follow (P_lookup (parent (fold G src s))) v) = rev (follow ?u) @ [v]"
-    using cond Q_head_queue_not_white
-    by (simp add: not_white_imp_rev_follow_fold_eq_rev_follow)
-  thus "dpath_bet (G.E G) (rev (parent.follow (P_lookup (parent (fold G src s))) v)) src v"
-    using rev_follow_head_queue_shortest_dpath
-    using v_mem_out_neighborhood dpath_bet_transitive
-    by (fastforce simp add: G.mem_out_neighborhood_iff_edge edge_iff_dpath_bet)
-  hence "reachable (G.E G) src v"
-    by (auto simp add: reachable_iff_dpath_bet)
-  with cond True
-  have "dist G src v = dist G src ?u + 1"
-    using True not_white_fold
-    by (intro white_not_white_fold_imp(1) not_white_imp_shortest_dpath_fold_case_1_aux[symmetric])
-  also have "... = dpath_length (rev (follow ?u)) + 1"
-    unfolding plus_enat_simps(1)[symmetric]
-    by (simp add: rev_follow_head_queue_shortest_dpath)
-  also have "... = dpath_length (rev (parent.follow (P_lookup (parent (fold G src s))) v))"
-    using follow_non_empty
-    by (simp add: rev_follow_fold_eq dpath_length_snoc)
-  finally show "dpath_length (rev (parent.follow (P_lookup (parent (fold G src s))) v)) = dist G src v"
-    by simp
-next
-  case False
+lemma (in bfs_invar_not_DONE) d_triangle_inequality_fold:
+  assumes dpath_p: "dpath_bet (G.dE G) p u v"
+  assumes not_white_fold_u: "\<not> white (fold G src s) u"
+  assumes not_white_fold_v: "\<not> white (fold G src s) v"
+  shows "d (parent (fold G src s)) v \<le> d (parent (fold G src s)) u + dpath_length p"
+proof -
+  consider
+    (white_white) "white s u \<and> white s v" |
+    (white_not_white) "white s u \<and> \<not> white s v" |
+    (gray_white) "gray s u \<and> white s v" |
+    (black_white) "black s u \<and> white s v" |
+    (not_white_not_white) "\<not> white s u \<and> \<not> white s v"
+    by fast
   thus ?thesis
-    using cond not_white_imp_shortest_dpath
-    by (simp add: not_white_imp_rev_follow_fold_eq_rev_follow)
-qed
+  proof (cases)
+    case white_white
+    hence "d (parent (fold G src s)) v = d (parent (fold G src s)) (Q_head (queue s)) + 1"
+      using not_white_fold_v
+      by (intro white_not_white_foldD(3)) simp
+    also have "... = d (parent (fold G src s)) u"
+      using white_white not_white_fold_u
+      by (intro white_not_white_foldD(3)[symmetric]) simp
+    finally show ?thesis
+      by simp
+  next
+    case white_not_white
+    hence dpath_Cons: "dpath_bet (G.dE G) (Q_head (queue s) # p) (Q_head (queue s)) v"
+      using not_white_fold_u white_not_white_foldD(1) dpath_p
+      by (auto simp add: G.mem_adjacency_iff_edge intro: dpath_bet_Cons_edge)
+    have "d (parent (fold G src s)) v = d (parent s) v"
+      using white_not_white
+      by (simp add: not_whiteD(3))
+    also have "... \<le> d (parent s) (Q_head (queue s)) + dpath_length (Q_head (queue s) # p)"
+      using not_white_head_queue white_not_white dpath_Cons
+      by (auto intro: d_triangle_inequality)
+    also have "... = d (parent s) (Q_head (queue s)) + 1 + dpath_length p"
+      using dpath_p
+      by (simp add: dpath_length_Cons)
+    also have "... = d (parent (fold G src s)) (Q_head (queue s)) + 1 + dpath_length p"
+      using not_white_head_queue
+      by (simp add: not_whiteD(3))
+    also have "... = d (parent (fold G src s)) u + dpath_length p"
+      using white_not_white not_white_fold_u
+      by (simp add: white_not_white_foldD(3))
+    finally show ?thesis
+      .
+  next
+    case gray_white
+    hence "d (parent (fold G src s)) v = d (parent (fold G src s)) (Q_head (queue s)) + 1"
+      using not_white_fold_v
+      by (intro white_not_white_foldD(3)) simp
+    also have "... = d (parent s) (Q_head (queue s)) + 1"
+      using not_white_head_queue
+      by (auto simp add: not_whiteD(3))
+    also have "... \<le> d (parent s) u + 1"
+      using gray_white
+      by (intro mem_queue_imp_d_ge add_right_mono) simp
+    also have "... = d (parent (fold G src s)) u + 1"
+      using gray_white
+      by (simp add: not_whiteD(3))
+    also have "... \<le> d (parent (fold G src s)) u + dpath_length p"
+      using dpath_p gray_white
+      by (fastforce intro: dpath_length_hd_noteq_last add_left_mono)
+    finally show ?thesis
+      .
+  next
+    case black_white
+    then obtain w where
+      "w \<in> set p" and
+      gray_w: "gray s w"
+      using dpath_p
+      by (elim white_imp_gray_ancestor) simp+
+    then obtain q r where
+      "p = q @ tl r" and
+      dpath_q: "dpath_bet (G.dE G) q u w" and
+      dpath_r: "dpath_bet (G.dE G) r w v"
+      using dpath_p
+      by (auto simp add: in_set_conv_decomp elim: dpath_bet_vertex_decompE)
+    hence dpath_length_p: "dpath_length p = dpath_length q + dpath_length r"
+      by (auto dest: dpath_betD(2-4) intro: dpath_length_append_2)
 
-subsubsection \<open>@{thm bfs_invar.black_imp_out_neighborhood_not_white}\<close>
-
-lemma (in bfs_invar) black_imp_out_neighborhood_not_white_fold:
-  assumes cond: "cond s"
-  assumes black_fold: "black (fold G src s) v"
-  shows "\<forall>w\<in>set (G.out_neighborhood G v). \<not> white (fold G src s) w"
-proof (induct s v rule: vertex_color_induct)
-  case white
-  hence "v \<in> set (G.out_neighborhood G (Q_head (queue s)))"
-    using assms
-    by (intro white_not_white_fold_imp(1)) simp+
-  hence "v \<in> set (Q_list (queue (fold G src s)))"
-    using white cond
-    by (simp add: discovered_def list_queue_fold_cong)
-  thus ?case
-    using black_fold
-    by blast
-next
-  case gray
-  hence "v = Q_head (queue s)"
-    using assms queue_invar
-    by (intro head_queue_if) simp+
-  thus ?case
-    by (auto simp add: discovered_def lookup_parent_fold_cong override_on_def)
-next
-  case black
-  hence "\<forall>w\<in>set (G.out_neighborhood G v). \<not> white s w"
-    by (intro black_imp_out_neighborhood_not_white)
-  thus ?case
-    using not_white_imp_not_white_fold
-    by blast
+    have "d (parent (fold G src s)) v = d (parent (fold G src s)) (Q_head (queue s)) + 1"
+      using black_white not_white_fold_v
+      by (intro white_not_white_foldD(3)) simp
+    also have "... = d (parent s) (Q_head (queue s)) + 1"
+      using not_white_head_queue
+      by (auto simp add: not_whiteD(3))
+    also have "... \<le> d (parent s) w + 1"
+      using gray_w
+      by (intro mem_queue_imp_d_ge add_right_mono) simp
+    also have "... \<le> d (parent s) u + dpath_length q + 1"
+      using dpath_q black_white gray_w
+      by (auto intro: d_triangle_inequality add_right_mono)
+    also have "... \<le> d (parent s) u + dpath_length p"
+      using dpath_r gray_w black_white dpath_length_hd_noteq_last
+      by (fastforce simp add: dpath_length_p)
+    also have "... = d (parent (fold G src s)) u + dpath_length p"
+      using black_white
+      by (simp add: not_whiteD(3))
+    finally show ?thesis
+      .
+  next
+    case not_white_not_white
+    hence "d (parent (fold G src s)) v = d (parent s) v"
+      by (simp add: not_whiteD(3))
+    also have "... \<le> d (parent s) u + dpath_length p"
+      using dpath_p not_white_not_white
+      by (intro d_triangle_inequality) simp+
+    also have "... = d (parent (fold G src s)) u + dpath_length p"
+      using not_white_not_white
+      by (simp add: not_whiteD(3))
+    finally show ?thesis
+      .
+  qed
 qed
 
 subsubsection \<open>\<close>
 
-lemma (in bfs_invar) bfs_invar_fold:
-  assumes "cond s"
+lemma (in bfs_invar_not_DONE) bfs_invar_fold:
   shows "bfs_invar'' (fold G src s)"
-  using assms
-  using bfs_axioms
-  using follow_invar'_parent_fold
-  using queue_invar_fold queue_distinct_fold parent_invar_fold parent_src_fold
-  using gray_if_mem_queue_fold black_if_mem_ran_fold queue_sorted_wrt_dpath_length_fold tbd_dpath_length_fold
-  using not_white_imp_shortest_dpath_fold black_imp_out_neighborhood_not_white_fold
-  by unfold_locales
-
-subsection \<open>@{term bfs.loop}\<close>
-
-lemma (in bfs) loop_psimps:
-  assumes "bfs_invar' G src s"
-  shows "loop G src s = (if cond s then loop G src (fold G src s) else s)"
-proof -
-  have "G.invar G"
-    using assms
-    by (intro bfs_invar.axioms(1) bfs_invar_tbd.G_invar)
-  moreover have "Q_invar (queue s)"
-    using assms
-    by (intro bfs_invar.queue_invar)
-  moreover have "P_invar (parent s)"
-    using assms
-    by (intro bfs_invar.parent_invar)
-  moreover have "set (Q_list (queue s)) \<subseteq> G.V G"
-    using assms
-    by (intro bfs_invar.queue_subset_V)
-  moreover have "P.dom (parent s) \<subseteq> G.V G"
-    using assms
-    by (intro bfs_invar.dom_parent_subset_V)
-  ultimately show ?thesis
-    by (metis loop_dom loop.psimps)
+proof (standard, goal_cases)
+  case 1
+  show ?case using follow_invar'_parent_fold .
+next
+  case 2
+  show ?case using invar_queue_fold .
+next
+  case 3
+  show ?case using invar_parent_fold .
+next
+  case 4
+  show ?case using parent_src_fold .
+next
+  case (5 v u)
+  thus ?case by (intro parent_imp_edge_fold)
+next
+  case (6 v)
+  thus ?case by (intro not_white_if_mem_queue_fold)
+next
+  case (7 v u)
+  thus ?case by (intro not_white_if_parent_fold)
+next
+  case (8 u v)
+  thus ?case by (intro black_imp_adjacency_not_white_fold)
+next
+  case 9
+  show ?case using queue_sorted_wrt_d_fold .
+next
+  case 10
+  thus ?case by (intro d_last_queue_le_fold)
+next
+  case (11 p u v)
+  thus ?case by (intro d_triangle_inequality_fold)
 qed
-
-lemma (in bfs) bfs_induct:
-  assumes "bfs_invar' G src s"
-  assumes "\<And>G src s. loop_dom (G, src, s) \<Longrightarrow> (cond s \<Longrightarrow> P G src (fold G src s)) \<Longrightarrow> P G src s"
-  shows "P G src s"
-proof -
-  have "G.invar G"
-    using assms(1)
-    by (intro bfs_invar.axioms(1) bfs_invar_tbd.G_invar)
-  moreover have "Q_invar (queue s)"
-    using assms(1)
-    by (intro bfs_invar.queue_invar)
-  moreover have "P_invar (parent s)"
-    using assms(1)
-    by (intro bfs_invar.parent_invar)
-  moreover have "set (Q_list (queue s)) \<subseteq> G.V G"
-    using assms
-    by (intro bfs_invar.queue_subset_V)
-  moreover have "P.dom (parent s) \<subseteq> G.V G"
-    using assms(1)
-    by (intro bfs_invar.dom_parent_subset_V)
-  ultimately show ?thesis
-    using assms(2)
-    by (blast intro: loop_dom loop.pinduct)
-qed
-
-lemma (in bfs) bfs_invar_loop:
-  assumes "bfs_invar' G src s"
-  shows "bfs_invar' G src (loop G src s)"
-  using assms
-proof (induct rule: bfs_induct[OF assms])
-  case (1 G src s)
-  thus ?case
-    by (fastforce simp add: loop_psimps intro: bfs_invar.bfs_invar_fold)
-qed
-
-subsection \<open>@{term bfs}\<close>
-
-lemma (in bfs_invar_tbd) bfs_invar_bfs:
-  shows "bfs_invar'' (bfs G src)"
-  using bfs_invar_init
-  by (intro bfs_invar_loop)
 
 section \<open>Correctness\<close>
 
-lemma (in bfs_invar_tbd) soundness:
-  assumes "bfs_invar'' s"
-  assumes "discovered src (loop G src s) v"
-  shows "is_shortest_dpath G (rev (parent.follow (P_lookup (parent (loop G src s))) v)) src v"
-  using assms bfs_invar_loop bfs_invar.not_white_imp_shortest_dpath
-  by fast
+subsection \<open>Definitions\<close>
+
+abbreviation (in bfs) dist :: "'n \<Rightarrow> 'a \<Rightarrow> 'a \<Rightarrow> enat" where
+  "dist G \<equiv> Shortest_Dpath.dist (G.dE G)"
+
+abbreviation (in bfs) shortest_dpath :: "'n \<Rightarrow> 'a list \<Rightarrow> 'a \<Rightarrow> 'a \<Rightarrow> bool" where
+  "shortest_dpath G p u v \<equiv> dpath_bet (G.dE G) p u v \<and> dpath_length p = dist G u v"
+
+subsection \<open>Basic Lemmas\<close>
+
+lemma (in bfs_invar) queue_subset_dV:
+  shows "set (Q_list (queue s)) \<subseteq> G.dV G"
+  using not_white_if_mem_queue not_white_imp_dpath_rev_follow
+  by (auto intro: dpath_bet_endpoints(2))
+
+lemma (in bfs_invar) dom_parent_subset_dV:
+  shows "P.dom (parent s) \<subseteq> G.dV G"
+proof
+  fix v
+  assume "v \<in> P.dom (parent s)"
+  then obtain u where
+    "P_lookup (parent s) v = Some u"
+    by (auto simp add: P.dom_def)
+  hence "(u, v) \<in> G.dE G"
+    by (intro parent_imp_edge)
+  thus "v \<in> G.dV G"
+    by (intro G.edgeI(2))
+qed
+
+subsection \<open>Convenience Lemmas\<close>
+
+lemma (in bfs_invar) loop_dom:
+  shows "loop_dom (G, src, s)"
+  using invar_G invar_queue invar_parent queue_subset_dV dom_parent_subset_dV
+  by (intro loop_dom)
+
+lemma (in bfs) loop_psimps:
+  assumes "bfs_invar' G src s"
+  shows "loop G src s = (if \<not> DONE s then loop G src (fold G src s) else s)"
+  using assms
+  by (metis bfs_invar.loop_dom loop.psimps)
+
+lemma (in bfs_invar_not_DONE) loop_psimps:
+  shows "loop G src s = loop G src (fold G src s)"
+  using not_DONE bfs_invar_axioms
+  by (simp add: loop_psimps)
+
+lemma (in bfs_invar_DONE) loop_psimps:
+  shows "loop G src s = s"
+  using DONE bfs_invar_axioms
+  by (simp add: loop_psimps)
+
+lemma (in bfs) bfs_induct:
+  assumes "bfs_invar' G src s"
+  assumes "\<And>G src s. loop_dom (G, src, s) \<Longrightarrow> (\<not> DONE s \<Longrightarrow> P G src (fold G src s)) \<Longrightarrow> P G src s"
+  shows "P G src s"
+  using assms
+  by (blast intro: bfs_invar.loop_dom loop.pinduct)
+
+subsection \<open>Completeness\<close>
+
+lemma (in bfs_invar_DONE) white_imp_not_reachable:
+  assumes "white s v"
+  shows "\<not> reachable (G.dE G) src v"
+proof
+  assume "reachable (G.dE G) src v"
+  then obtain p where
+    "dpath_bet (G.dE G) p src v"
+    unfolding reachable_iff_dpath_bet
+    ..
+  thus False
+    using assms
+  proof (induct p arbitrary: v rule: dpath_rev_induct)
+    case 1
+    thus ?case
+      by simp
+  next
+    case 2
+    thus ?case
+      using src_not_white hd_of_dpath_bet' last_of_dpath_bet
+      by fastforce
+  next
+    case (3 u u' l)
+    show ?case
+    proof (induct s u rule: vertex_color_induct)
+      case white
+      have "dpath_bet (G.dE G) (l @ [u]) src u"
+        using "3.prems"(1)
+        by (intro dpath_bet_pref) simp
+      thus ?case
+        using white
+        by (intro "3.hyps")
+    next
+      case gray
+      thus ?case
+        using invar_queue DONE
+        by (simp add: Q.is_empty DONE_def)
+    next
+      case black
+      have "(u, v) \<in> G.dE G"
+        using "3.prems"(1)
+        by (auto simp add: dpath_bet_def intro: dpath_snoc_edge_2)
+      thus ?case
+        using black black_imp_adjacency_not_white "3.prems"(2)
+        by blast
+    qed
+  qed
+qed
 
 lemma (in bfs_invar_tbd) completeness:
   assumes "bfs_invar'' s"
-  assumes "\<not> discovered src (loop G src s) v"
-  shows "\<not> reachable (G.E G) src v"
+  assumes "\<not> discovered src (parent (loop G src s)) v"
+  shows "\<not> reachable (G.dE G) src v"
   using assms
 proof (induct rule: bfs_induct[OF assms(1)])
   case (1 G src s)
   show ?case
-  proof (cases "cond s")
+  proof (cases "DONE s")
     case True
+    with "1.prems"(1)
+    have "bfs_invar_DONE' G src s"
+      by (intro bfs_invar_DONE'I)
     thus ?thesis
-      using "1.prems"
-      by (intro bfs_invar.bfs_invar_fold "1.hyps"(2)) (simp_all add: loop_psimps)
+      using "1.prems"(2)
+      by (intro bfs_invar_DONE.white_imp_not_reachable) (simp_all add: bfs_invar_DONE.loop_psimps)
   next
     case False
-    hence "\<not> discovered src s v"
-      using "1.prems"
-      by (simp add: loop_psimps)
-    from bfs_invar.white_imp_dist_ge[OF "1.prems"(1) this]
-    have "dist G src v = \<infinity>"
-      using "1.prems"(1) False bfs_invar.white_imp_dist_ge
-      by (fastforce simp add: cond_def)
+    with "1.prems"(1)
+    have "bfs_invar_not_DONE' G src s"
+      by (intro bfs_invar_not_DONE'I)
     thus ?thesis
-      using dist_eq_\<delta> \<delta>_reachable_conv
-      by metis
+      using False "1.prems"(2)
+      by (intro bfs_invar_not_DONE.bfs_invar_fold "1.hyps"(2)) (simp_all add: bfs_invar_not_DONE.loop_psimps)
   qed
 qed
 
-abbreviation (in bfs) is_shortest_dpath_Map :: "'n \<Rightarrow> 'a \<Rightarrow> ('q, 'm) state \<Rightarrow> bool" where
-  "is_shortest_dpath_Map G src s \<equiv>
-   \<forall>v. 
-    discovered src s v \<longrightarrow> is_shortest_dpath G (rev (parent.follow (P_lookup (parent s)) v)) src v \<and>
-    \<not> discovered src s v \<longrightarrow> \<not> reachable (G.E G) src v"
+subsection \<open>Soundness\<close>
+
+lemma (in bfs_invar_DONE) not_white_imp_d_le_dist:
+  assumes "\<not> white s v"
+  shows "d (parent s) v \<le> dist G src v"
+proof -
+  have "reachable (G.dE G) src v"
+    using assms
+    by (auto simp add: reachable_iff_dpath_bet intro: not_white_imp_dpath_rev_follow)
+  then obtain p where
+    "shortest_dpath G p src v"
+    by (elim dist_dpath_betE) simp+
+  thus ?thesis
+    using assms
+  proof (induct p arbitrary: v rule: dpath_rev_induct)
+    case 1
+    thus ?case
+      by simp
+  next
+    case 2
+    thus ?case
+      using parent_src hd_of_dpath_bet' last_of_dpath_bet
+      by (fastforce simp add: follow_psimps intro: list_length_1)
+  next
+    case (3 u u' l)
+    show ?case
+    proof (cases "white s u")
+      case True
+      hence "dist G src u = \<infinity>"
+        by (metis white_imp_not_reachable dist_eq_\<delta> \<delta>_reachable_conv)
+      thus ?thesis
+        using "3.prems"(1)
+        by (auto intro: shortest_dpathE_2)
+    next
+      case False
+      have shortest_dpath: "shortest_dpath G (l @ [u]) src u"
+        using "3.prems"(1)
+        by
+          (auto
+           simp add: dpath_length_eq_dpath_weight dist_eq_\<delta> shortest_dpath_def[symmetric]
+           intro: shortest_dpath_prefix_shortest_dpath)
+      have "(u, v) \<in> G.dE G"
+        using "3.prems"(1) last_of_dpath_bet
+        by (fastforce simp add: edge_iff_dpath_bet intro: split_dpath)
+      hence "d (parent s) v \<le> d (parent s) u + 1"
+        using False "3.prems"(2)
+        by (intro d_triangle_inequality_edge)
+      also have "... \<le> dist G src u + 1"
+        using "3.hyps"[OF shortest_dpath False]
+        unfolding plus_enat_simps(1)[symmetric] one_enat_def[symmetric]
+        by (intro add_right_mono)
+      also have "... = dist G src v"
+        using "3.prems"(1)
+        by (auto intro: shortest_dpathE_2)
+      finally show ?thesis
+        by simp
+    qed
+  qed
+qed
+
+lemma (in bfs_invar_DONE) not_white_imp_shortest_dpath:
+  assumes "\<not> white s v"
+  shows "shortest_dpath G (rev_follow (parent s) v) src v"
+proof (rule conjI)
+  show "dpath_bet (G.dE G) (rev_follow (parent s) v) src v"
+    using assms
+    by (intro not_white_imp_dpath_rev_follow)
+  thus "d (parent s) v = dist G src v"
+    using assms
+    by (intro not_white_imp_d_le_dist dist_le_dpath_length antisym)
+qed
+
+lemma (in bfs_invar_tbd) soundness:
+  assumes "bfs_invar'' s"
+  assumes "discovered src (parent (loop G src s)) v"
+  shows "shortest_dpath G (rev_follow (parent (loop G src s)) v) src v"
+  using assms
+proof (induct rule: bfs_induct[OF assms(1)])
+  case (1 G src s)
+  show ?case
+  proof (cases "DONE s")
+    case True
+    with "1.prems"(1)
+    have "bfs_invar_DONE' G src s"
+      by (intro bfs_invar_DONE'I)
+    thus ?thesis
+      using "1.prems"(2)
+      by (intro bfs_invar_DONE.not_white_imp_shortest_dpath) (simp_all add: bfs_invar_DONE.loop_psimps)
+  next
+    case False
+    with "1.prems"(1)
+    have "bfs_invar_not_DONE' G src s"
+      by (intro bfs_invar_not_DONE'I)
+    thus ?thesis
+      using False "1.prems"(2)
+      by (auto simp add: bfs_invar_not_DONE.loop_psimps dest: "1.hyps"(2) intro: bfs_invar_not_DONE.bfs_invar_fold)
+  qed
+qed
+
+subsection \<open>Correctness\<close>
+
+abbreviation (in bfs) shortest_dpath_Map :: "'n \<Rightarrow> 'a \<Rightarrow> 'm \<Rightarrow> bool" where
+  "shortest_dpath_Map G src m \<equiv>
+   \<forall>v. (discovered src m v \<longrightarrow> shortest_dpath G (rev_follow m v) src v) \<and>
+       (\<not> discovered src m v \<longrightarrow> \<not> reachable (G.dE G) src v)"
 
 lemma (in bfs_invar_tbd) correctness:
   assumes "bfs_invar'' s"
-  shows "is_shortest_dpath_Map G src (loop G src s)"
+  shows "shortest_dpath_Map G src (parent (loop G src s))"
   using assms soundness completeness
-  by simp+
+  by simp
 
 theorem (in bfs_invar_tbd) bfs_correct:
-  shows "is_shortest_dpath_Map G src (bfs G src)"
-  using bfs_invar_init correctness
-  by simp+
+  shows "shortest_dpath_Map G src (bfs G src)"
+  using bfs_invar_init
+  by (intro correctness)
 
 corollary (in bfs) bfs_correct:
   assumes "bfs_invar_tbd' G src"
-  shows "is_shortest_dpath_Map G src (bfs G src)"
+  shows "shortest_dpath_Map G src (bfs G src)"
   using assms
   by (intro bfs_invar_tbd.bfs_correct)
 
