Graph_Theory/Undirected_Graphs/Augmenting_Path.thy
@@ -23,6 +23,41 @@ lemma augmenting_pathI:
   using assms
   by (simp add: augmenting_path_def)
 
+lemma augmenting_path_rev_if_augmenting_path:
+  assumes "augmenting_path M p"
+  shows "augmenting_path M (rev p)"
+proof (rule augmenting_pathI, goal_cases)
+  case 1
+  show ?case
+    using assms
+    by (auto dest: augmenting_pathD(1))
+next
+  case 2
+  show ?case
+    using assms
+    by
+      (auto
+       simp add: edges_of_path_rev[symmetric]
+       dest: augmenting_pathD(2) augmenting_path_odd_length
+       intro: alt_list_rev)
+next
+  case 3
+  have "p \<noteq> []"
+    using assms
+    by (auto dest: augmenting_pathD(1))
+  thus ?case
+    using assms
+    by (auto simp add: hd_rev dest: augmenting_pathD(4))
+next
+  case 4
+  have "p \<noteq> []"
+    using assms
+    by (auto dest: augmenting_pathD(1))
+  thus ?case
+    using assms
+    by (auto simp add: last_rev dest: augmenting_pathD(3))
+qed
+
 term augpath
 lemma augpathD:
   assumes "augpath G M p"
@@ -40,5 +75,25 @@ lemma augpathI:
   shows "augpath G M p"
   using assms
   by simp
+
+lemma augpath_rev_if_augpath:
+  assumes "augpath G M p"
+  shows "augpath G M (rev p)"
+proof (rule augpathI, goal_cases)
+  case 1
+  show ?case
+    using assms
+    by (intro rev_path_is_path) simp
+next
+  case 2
+  show ?case
+    using assms
+    by force
+next
+  case 3
+  show ?case
+    using assms
+    by (intro augmenting_path_rev_if_augmenting_path) simp
+qed
 
 end
