Map_Specs_Tbd.thy
@@ -14,7 +14,7 @@ lemma (in Map) mem_dom_iff:
 definition (in Map) ran :: "'m \<Rightarrow> 'b set" where
   "ran m \<equiv> {b. \<exists>a. lookup m a = Some b}"
 
-lemma (in Map) dom_finite_imp_ran_finite:
+lemma (in Map) finite_dom_imp_finite_ran:
   assumes "finite (dom m)"
   shows "finite (ran m)"
 proof -
@@ -105,16 +105,194 @@ proof -
     by blast
 qed
 
-lemma (in Map_by_Ordered) dom_finite:
+lemma (in Map_by_Ordered) finite_dom:
   assumes "invar m"
   shows "finite (dom m)"
   using assms
   by (simp add: dom_inorder_cong)
 
-lemma (in Map_by_Ordered) ran_finite:
+lemma (in Map_by_Ordered) finite_ran:
   assumes "invar m"
   shows "finite (ran m)"
   using assms
-  by (intro dom_finite dom_finite_imp_ran_finite)
+  by (intro finite_dom finite_dom_imp_finite_ran)
+
+(**)
+lemma (in Map_by_Ordered) set_filter_inorder_cong:
+  assumes "invar m"
+  shows "set (filter (\<lambda>p. fst p = a) (inorder m)) = (case lookup m a of None \<Rightarrow> {} | Some b \<Rightarrow> {(a, b)})"
+proof -
+  { fix p
+    have "p \<in> set (filter (\<lambda>p. fst p = a) (inorder m)) \<longleftrightarrow> (\<exists>b. (a, b) \<in> set (inorder m) \<and> p = (a, b))"
+      unfolding filter_set[symmetric] member_filter
+      by (auto simp add: eq_fst_iff)
+    also have "... \<longleftrightarrow> (\<exists>b. lookup m a = Some b \<and> p = (a, b))"
+      using assms
+      by (simp add: mem_inorder_iff_lookup_eq_Some)
+    also have "... \<longleftrightarrow> p \<in> (case lookup m a of None \<Rightarrow> {} | Some b \<Rightarrow> {(a, b)})"
+      by (simp split: option.split)
+    finally have "p \<in> set (filter (\<lambda>p. fst p = a) (inorder m)) \<longleftrightarrow> p \<in> (case lookup m a of None \<Rightarrow> {} | Some b \<Rightarrow> {(a, b)})"
+      . }
+  thus ?thesis
+    by simp
+qed
+
+(**)
+lemma sorted1D:
+  assumes "sorted (a # map fst ps)"
+  shows "(a, y) \<notin> set ps"
+proof -
+  have "map_of ps a = None"
+    using assms
+    by (intro map_of_None) simp
+  thus ?thesis
+    using assms
+    by (auto simp add: map_of_eq_Some_iff_mem[symmetric] dest: sorted_cons)
+qed
+
+lemma sorted1D_2:
+  assumes "sorted (a # map fst ps)"
+  assumes "x < a"
+  shows "(x, y) \<notin> set ps"
+proof -
+  have "map_of ps x = None"
+    using assms
+    by (intro map_of_sorted_Cons) simp
+  thus ?thesis
+    using assms
+    by (auto simp add: map_of_eq_Some_iff_mem[symmetric] dest: sorted_cons)
+qed
+
+(**)
+lemma set_del_list_cong:
+  assumes "sorted1 l"
+  shows "set (del_list x l) = set l - set (filter (\<lambda>p. fst p = x) l)"
+  using assms
+proof (induct l rule: del_list.induct)
+  case (1 x)
+  thus ?case
+    by simp
+next
+  case (2 x a b ps)
+  show ?case
+  proof (cases "x = a")
+    case True
+    hence "set (del_list x ((a, b) # ps)) = set ps"
+      by simp
+    also have "... = set ((a, b) # ps) - {(a, b)}"
+      using "2.prems"
+      by (auto dest: sorted1D)
+    also have "... = set ((a, b) # ps) - set (filter (\<lambda>p. fst p = x) ((a, b) # ps))"
+      using "2.prems" True
+      by (auto dest: sorted1D)
+    finally show ?thesis
+      .
+  next
+    case False
+    hence "set (del_list x ((a, b) # ps)) = set ((a, b) # del_list x ps)"
+      by simp
+    also have "... = {(a, b)} \<union> set (del_list x ps)"
+      by force
+    also have "... = {(a, b)} \<union> set ps - set (filter (\<lambda>p. fst p = x) ps)"
+      using False "2.prems"
+      by (subst "2.hyps") (auto dest: sorted_cons)
+    also have "... = set ((a, b) # ps) - set (filter (\<lambda>p. fst p = x) ((a, b) # ps))"
+      using False
+      by force
+    finally show ?thesis
+      .
+  qed
+qed
+
+lemma (in Map_by_Ordered) set_inorder_delete_cong:
+  assumes "invar m"
+  shows "set (inorder (delete a m)) = set (inorder m) - (case lookup m a of None \<Rightarrow> {} | Some b \<Rightarrow> {(a, b)})"
+proof -
+  have "set (inorder (delete a m)) = set (del_list a (inorder m))"
+    using assms
+    by (simp add: invar_def inorder_delete)
+  also have "... = set (inorder m) - set (filter (\<lambda>p. fst p = a) (inorder m))"
+    using assms
+    by (simp add: invar_def set_del_list_cong)
+  also have "... = set (inorder m) - (case lookup m a of None \<Rightarrow> {} | Some b \<Rightarrow> {(a, b)})"
+    unfolding set_filter_inorder_cong[OF assms]
+    ..
+  finally show ?thesis
+    .
+qed
+
+(**)
+lemma set_upd_list_cong:
+  assumes "sorted1 l"
+  shows "set (upd_list x y l) = set l - set (filter (\<lambda>p. fst p = x) l) \<union> {(x, y)}"
+  using assms
+proof (induct l rule: upd_list.induct)
+  case (1 x y)
+  thus ?case
+    by simp
+next
+  case (2 x y a b ps)
+  consider (l) "x < a" | (e) "x = a" | (g) "x > a"
+    by fastforce
+  thus ?case
+  proof (cases)
+    case l
+    have "set (upd_list x y ((a, b) # ps)) = set ((x, y) # (a, b) # ps)"
+      using l
+      by simp
+    also have "... = set ((a, b) # ps) \<union> {(x, y)}"
+      by simp
+    also have "... = set ((a, b) # ps) - set (filter (\<lambda>p. fst p = x) ((a, b) # ps)) \<union> {(x, y)}"
+      using "2.prems" l
+      by (auto simp add: filter_empty_conv dest: sorted1D_2)
+    finally show ?thesis
+      .
+  next
+    case e
+    hence "set (upd_list x y ((a, b) # ps)) = set ((x, y) # ps)"
+      by simp
+    also have "... = set ps \<union> {(x, y)}"
+      by simp
+    also have "... = set ((a, b) # ps) - {(a, b)} \<union> {(x, y)}"
+      using "2.prems"
+      by (auto dest: sorted1D)
+    also have "... = set ((a, b) # ps) - set (filter (\<lambda>p. fst p = x) ((a, b) # ps)) \<union> {(x, y)}"
+      using "2.prems" e
+      by (auto dest: sorted1D)
+    finally show ?thesis
+      .
+  next
+    case g
+    hence "set (upd_list x y ((a, b) # ps)) = set ((a, b) # upd_list x y ps)"
+      by force
+    also have "... = {(a, b)} \<union> set (upd_list x y ps)"
+      by force
+    also have "... = {(a, b)} \<union> set ps - set (filter (\<lambda>p. fst p = x) ps) \<union> {(x, y)}"
+      using g "2.prems"
+      by (subst "2.hyps") (auto dest: sorted_cons)
+    also have "... = set ((a, b) # ps) - set (filter (\<lambda>p. fst p = x) ((a, b) # ps)) \<union> {(x, y)}"
+      using g
+      by force
+    finally show ?thesis
+    .
+  qed
+qed
+
+lemma (in Map_by_Ordered) set_inorder_update_cong:
+  assumes "invar m"
+  shows "set (inorder (update a b m)) = set (inorder m) - (case lookup m a of None \<Rightarrow> {} | Some y \<Rightarrow> {(a, y)}) \<union> {(a, b)}"
+proof -
+  have "set (inorder (update a b m)) = set (upd_list a b (inorder m))"
+    using assms
+    by (simp add: invar_def inorder_update)
+  also have "... = set (inorder m) - set (filter (\<lambda>p. fst p = a) (inorder m)) \<union> {(a, b)}"
+    using assms
+    by (simp add: invar_def set_upd_list_cong)
+  also have "... = set (inorder m) - (case lookup m a of None \<Rightarrow> {} | Some y \<Rightarrow> {(a, y)}) \<union> {(a, b)}"
+    unfolding set_filter_inorder_cong[OF assms]
+    ..
+  finally show ?thesis
+    .
+qed
 
 end
